fairness/examples/comp/comp.v
@@ -9,38 +9,31 @@ From iris.prelude Require Import options.
 From iris.algebra Require Import excl_auth auth gmap gset excl.
 From iris.bi Require Import bi.
 From trillium.fairness Require Import lm_fair. 
-From trillium.fairness.examples.comp Require Import lib.
+From trillium.fairness.ext_models Require Import ext_models.
+From trillium.fairness.examples.comp Require Import lib lib_ext.
 From trillium.fairness.heap_lang Require Export lang lm_lsi_hl_wp tactics proofmode_lsi.
 
 Close Scope Z_scope.
 
 Section ClientDefs.
 
-  (* TODO: generalize to any LSI_True model *)
-  Instance lib_model_inh: Inhabited (lm_ls lib_model).
-  Proof. 
-    pose proof (fmrole_inhabited lib_model_impl) as [ρ].
-    pose proof (fmstate_inhabited lib_model_impl) as [s].
-    eapply populate, (initial_ls s ρ). done.
-  Qed. 
-
-  Definition lib_fair := LM_Fair (LM := lib_model). 
-
   Let lib_st := fmstate lib_fair.
-  Let lib_role := fmrole lib_fair.
+  (* Let lib_role := fmrole lib_fair. *)
+  Let lib_erole := @ext_role _ ExtLibLM. 
 
   Definition client_state: Type := lib_st * nat.
 
   Inductive y_role := ρy.
-  Definition client_role: Type := lib_role + y_role.
+  Definition client_role: Type := lib_erole + y_role.
   
   Inductive client_trans: client_state -> option client_role -> client_state -> Prop :=
-  | ct_y_step_2 lb:
-    client_trans (lb, 2) (Some $ inr ρy) (lb, 1)
+  | ct_y_step_3 lb:
+    client_trans (lb, 3) (Some $ inr ρy) (lb, 2)
   (* TODO: allow arbitrary library's LM roles *)
-  | ct_lib_step lb1 lb2
-                (LIB_STEP: fmtrans lib_fair lb1 (Some ρlg) lb2):
-    client_trans (lb1, 1) (Some $ inl ρlg) (lb2, 1)
+  | ct_lib_ext lb1 lb2 (LIB_EXT: reset_lm_st_rel ρlg lb1 lb2):
+    client_trans (lb1, 2) (Some $ inl $ inr $ env (eiG ρlg) (EM := ExtLibLM)) (lb2, 1)
+  | ct_lib_step lb1 lb2 (LIB_STEP: fmtrans lib_fair lb1 (Some ρlg) lb2):
+    client_trans (lb1, 1) (Some $ inl $ inl ρlg) (lb2, 1)
   | ct_y_step_1 (lb: fmstate lib_fair)
                 (* (LIB_NOSTEP: 0 ∉ live_roles _ lb) *)
                 (LIB_NOROLES: ls_tmap lb (LM := lib_model) !! ρlg = Some ∅)
@@ -48,12 +41,13 @@ Section ClientDefs.
     client_trans (lb, 1) (Some $ inr ρy) (lb, 0)
   .
 
-  Global Instance lib_role_EqDec: EqDecision lib_role.
-  Proof. solve_decision. Defined.
-  Global Instance lib_role_Cnt: Countable lib_role.
-  Proof using. rewrite /lib_role. simpl. apply _. Defined.
+  (* Global Instance lib_role_EqDec: EqDecision lib_erole. *)
+  (* Proof. solve_decision. Defined. *)
+  (* Global Instance lib_role_Cnt: Countable lib_erole. *)
+  (* Proof using. *)
+  (*   rewrite /lib_erole. simpl. apply _.  *)
+  (* Defined. *)
   
-
   Instance y_EqDec: EqDecision y_role.
   Proof. by (solve_decision). Qed.
 
@@ -99,19 +93,30 @@ Section ClientDefs.
     Decision (exists st', client_trans st (Some ρ) st').
   Proof.
     Local Ltac nostep := right; intros [? T]; inversion T.
-    destruct st as [δ_lib n]. destruct n; [| destruct n]; [..| destruct n]. 
+    destruct st as [δ_lib n]. destruct n; [| destruct n]; [..| destruct n]; [..| destruct n]. 
     - by nostep. 
     - destruct ρ.
       + destruct l.
+        2: by nostep. 
+        destruct f. 
         destruct (decide (exists δ'_lib, locale_trans δ_lib () δ'_lib (LM := lib_model))).
-        * left. destruct e. eexists. econstructor. simpl. eauto.
-        * nostep. simpl in LIB_STEP. eauto. 
+        ** left. destruct e. eexists. econstructor. simpl. eauto.
+        ** nostep. simpl in LIB_STEP. eauto. 
       + destruct y. 
         destruct (ls_tmap δ_lib (LM := lib_model) !! ρlg) eqn:LIB_OBLS.
         2: { nostep. by rewrite LIB_OBLS in LIB_NOROLES. }
         destruct (decide (g = ∅)).
         * subst. left. eexists. by constructor. 
         * nostep. rewrite LIB_OBLS in LIB_NOROLES. set_solver.
+    - destruct ρ; [destruct l| ]. 
+      1, 3: by nostep. 
+      destruct e. destruct (decide (i ∈ active_exts δ_lib)).
+      + left. destruct i. 
+        apply active_exts_spec in e as [??]. simpl in *. 
+        eexists. destruct ρlg. 
+        eapply ct_lib_ext; eauto.
+      + nostep. subst. apply n. apply active_exts_spec.
+        inversion T. subst. simpl. eauto.
     - destruct ρ.
       + nostep.
       + destruct y. left. eexists. constructor.
@@ -119,18 +124,19 @@ Section ClientDefs.
   Qed.
 
   Definition client_lr (st: client_state): gset (client_role) :=
-    filter (fun r => (@bool_decide _ (lib_step_dec st r) = true))  {[ inl ρlg; inr ρy ]}. 
+    filter (fun r => (@bool_decide _ (lib_step_dec st r) = true))  
+      {[ inl $ inl ρlg; inl $ inr $ env (eiG ρlg) (EM := ExtLibLM); inr ρy ]}. 
 
   Lemma client_lr_spec: ∀ (s : client_state) (ρ : client_role),
       (exists s', client_trans s (Some ρ) s') <-> ρ ∈ client_lr s.
   Proof.
     intros ??. rewrite /client_lr.
     rewrite elem_of_filter. rewrite @bool_decide_eq_true.
-    rewrite elem_of_union. rewrite !elem_of_singleton. 
+    rewrite !elem_of_union. rewrite !elem_of_singleton. 
     split.
-    - intros [? TRANS]. split; eauto. inversion TRANS; subst; eauto.
-    - tauto. 
-  Qed. 
+    2: tauto. 
+    intros [? TRANS]. split; eauto. inversion TRANS; subst; eauto.
+  Qed.
 
   Definition client_model_impl: FairModel.
   Proof.
@@ -152,7 +158,7 @@ Section ClientDefs.
   Definition client_LSI (s: client_state)
     (m: gmap (fmrole client_model_impl) (locale heap_lang))
     (_: gmap (fmrole client_model_impl) nat) :=
-    forall gi, (exists ρi, ls_mapping s.1 !! ρi = Some gi) -> inl gi ∈ dom m.
+    forall gi, (exists ρi, ls_mapping s.1 !! ρi = Some gi) -> inl $ inl gi ∈ dom m.
     
   Definition client_fl := 15. 
   Definition client_model: LiveModel (locale heap_lang) client_model_impl client_LSI :=
@@ -200,818 +206,818 @@ Section ClientRA.
 End ClientRA.
 
 
-Section ClientSpec. 
-  Context `{EM: ExecutionModel heap_lang M} `{@heapGS Σ _ EM} {cpG: clientPreGS Σ}.
-  Context `{PMPP: @PartialModelPredicatesPre (locale heap_lang) _ _ Σ client_model_impl}.
+(* Section ClientSpec.  *)
+(*   Context `{EM: ExecutionModel heap_lang M} `{@heapGS Σ _ EM} {cpG: clientPreGS Σ}. *)
+(*   Context `{PMPP: @PartialModelPredicatesPre (locale heap_lang) _ _ Σ client_model_impl}. *)
 
-  (* Notation "'PMP'" := (fun Einvs => (PartialModelPredicates Einvs (EM := EM) (iLM := client_model) (PMPP := PMPP) (eGS := heap_fairnessGS))). *)
-  Notation "'LSG' Einvs" := (LM_steps_gen Einvs (EM := EM) (iLM := client_model) (PMPP := PMPP) (eGS := heap_fairnessGS)) (at level 10).
+(*   (* Notation "'PMP'" := (fun Einvs => (PartialModelPredicates Einvs (EM := EM) (iLM := client_model) (PMPP := PMPP) (eGS := heap_fairnessGS))). *) *)
+(*   Notation "'LSG' Einvs" := (LM_steps_gen Einvs (EM := EM) (iLM := client_model) (PMPP := PMPP) (eGS := heap_fairnessGS)) (at level 10). *)
 
-  (* TODO: remove tid=0 restriction ? *)
-  Let lib_pmi `{clientGS Σ} (m: gmap (locale heap_lang) (gset (fmrole lib_model_impl))): iProp Σ:=
-    (∃ (L: gset (fmrole lib_model_impl)) (Ract Rfr: gset client_role), 
-        ⌜ m = {[ 0 := L ]} ⌝ ∗
-         frag_mapping_is {[ ρlg := L ]} ∗
-         (⌜ L ≠ ∅ ⌝ ∗ ⌜ Ract = {[ inl ρlg ]} /\ Rfr = {[ inr ρy ]} ⌝ ∗ (∃ f: nat, partial_fuel_is {[ inl ρlg := f ]} ∗ ⌜ 1 <= f <= client_fl ⌝) ∨
-          ⌜ L = ∅ ⌝ ∗ ⌜ Ract = {[ inr ρy ]} /\ Rfr = {[ inl ρlg ]} ⌝ ∗ partial_fuel_is {[ inr ρy := client_fl ]}) ∗
-        partial_mapping_is {[ 0 := Ract ]} ∗
-        partial_free_roles_are Rfr ∗
-        y_frag_model_is 1). 
+(*   (* TODO: remove tid=0 restriction ? *) *)
+(*   Let lib_pmi `{clientGS Σ} (m: gmap (locale heap_lang) (gset (fmrole lib_model_impl))): iProp Σ:= *)
+(*     (∃ (L: gset (fmrole lib_model_impl)) (Ract Rfr: gset client_role),  *)
+(*         ⌜ m = {[ 0 := L ]} ⌝ ∗ *)
+(*          frag_mapping_is {[ ρlg := L ]} ∗ *)
+(*          (⌜ L ≠ ∅ ⌝ ∗ ⌜ Ract = {[ inl ρlg ]} /\ Rfr = {[ inr ρy ]} ⌝ ∗ (∃ f: nat, partial_fuel_is {[ inl ρlg := f ]} ∗ ⌜ 1 <= f <= client_fl ⌝) ∨ *)
+(*           ⌜ L = ∅ ⌝ ∗ ⌜ Ract = {[ inr ρy ]} /\ Rfr = {[ inl ρlg ]} ⌝ ∗ partial_fuel_is {[ inr ρy := client_fl ]}) ∗ *)
+(*         partial_mapping_is {[ 0 := Ract ]} ∗ *)
+(*         partial_free_roles_are Rfr ∗ *)
+(*         y_frag_model_is 1).  *)
   
-  Definition lib_PMPP `{clientGS Σ}:
-    @PartialModelPredicatesPre (locale heap_lang) _ _ Σ lib_model_impl.
-   refine
-    {|
-        partial_model_is := frag_model_is;
-        partial_free_roles_are := frag_free_roles_are;
-        partial_fuel_is := frag_fuel_is;
-        partial_mapping_is := lib_pmi;
-    |}.
-  Unshelve.
-  all: try (apply _ || solve_proper).
-  (* TODO: reuse proofs from resources.v *)
-  - intros. 
-    rewrite /frag_fuel_is.
-    rewrite map_fmap_union. rewrite -gmap_disj_op_union.
-    2: { by apply map_disjoint_fmap. }
-    by rewrite auth_frag_op own_op.
-  - intros. rewrite /frag_free_roles_are.
-    rewrite -gset_disj_union; auto.  
-    by rewrite auth_frag_op own_op.
-  - iApply own_unit.
-  Defined.
+(*   Definition lib_PMPP `{clientGS Σ}: *)
+(*     @PartialModelPredicatesPre (locale heap_lang) _ _ Σ lib_model_impl. *)
+(*    refine *)
+(*     {| *)
+(*         partial_model_is := frag_model_is; *)
+(*         partial_free_roles_are := frag_free_roles_are; *)
+(*         partial_fuel_is := frag_fuel_is; *)
+(*         partial_mapping_is := lib_pmi; *)
+(*     |}. *)
+(*   Unshelve. *)
+(*   all: try (apply _ || solve_proper). *)
+(*   (* TODO: reuse proofs from resources.v *) *)
+(*   - intros.  *)
+(*     rewrite /frag_fuel_is. *)
+(*     rewrite map_fmap_union. rewrite -gmap_disj_op_union. *)
+(*     2: { by apply map_disjoint_fmap. } *)
+(*     by rewrite auth_frag_op own_op. *)
+(*   - intros. rewrite /frag_free_roles_are. *)
+(*     rewrite -gset_disj_union; auto.   *)
+(*     by rewrite auth_frag_op own_op. *)
+(*   - iApply own_unit. *)
+(*   Defined. *)
 
-  Definition lib_spec_pre `{clientGS Σ} tid: iProp Σ := 
-    partial_model_is 1 (PartialModelPredicatesPre := lib_PMPP) ∗ 
-    has_fuels tid {[ ρl:=2 ]} (PMPP := lib_PMPP).
+(*   Definition lib_spec_pre `{clientGS Σ} tid: iProp Σ :=  *)
+(*     partial_model_is 1 (PartialModelPredicatesPre := lib_PMPP) ∗  *)
+(*     has_fuels tid {[ ρl:=2 ]} (PMPP := lib_PMPP). *)
 
-  Definition lib_spec_post `{clientGS Σ} tid: iProp Σ :=
-    partial_mapping_is {[ tid := ∅ ]} (PartialModelPredicatesPre := lib_PMPP) ∗ 
-    partial_free_roles_are {[ ρl ]} (PartialModelPredicatesPre := lib_PMPP). 
+(*   Definition lib_spec_post `{clientGS Σ} tid: iProp Σ := *)
+(*     partial_mapping_is {[ tid := ∅ ]} (PartialModelPredicatesPre := lib_PMPP) ∗  *)
+(*     partial_free_roles_are {[ ρl ]} (PartialModelPredicatesPre := lib_PMPP).  *)
 
-  Definition lib_ls_premise (lb: lm_ls lib_model) :=
-    ls_fuel lb !! ρl = Some 2 ∧ ls_under lb = 1 ∧ ls_tmap lb !! ρlg = Some {[ρl]}. 
+(*   Definition lib_ls_premise (lb: lm_ls lib_model) := *)
+(*     ls_fuel lb !! ρl = Some 2 ∧ ls_under lb = 1 ∧ ls_tmap lb !! ρlg = Some {[ρl]}.  *)
 
-  (* TODO: move to library, weaken Σ requirement *)
-  Lemma lib_premise_dis (lb: lm_ls lib_model)
-    (LB_INFO: lib_ls_premise lb):
-    ρlg ∈ live_roles lib_fair lb.
-  Proof. 
-    apply LM_live_roles_strong.
-    destruct LB_INFO as (F & S & TM).
-    eset (δ := ({| ls_under := (0: fmstate lib_model_impl); ls_fuel := ls_fuel lb; ls_mapping := ls_mapping lb; ls_inv := _ |})).     
-    exists δ. red. exists (Take_step ρl ρlg). split; [| done].    
-    repeat split; eauto.
-    - eapply ls_mapping_tmap_corr. eexists. split; eauto. set_solver.
-    - red. intros. inversion H2; subst; try set_solver.
-      destruct ρ', ρl; done.
-    - red. intros. left.
-      replace ρ' with ρl by (by destruct ρ', ρl). 
-      rewrite F. simpl. lia.
-    - intros. rewrite F. simpl. lia.
-    - intros. subst δ. simpl in H0. set_solver.
-    - subst δ. simpl. set_solver.
-    Unshelve.
-    + simpl. transitivity (∅: gset (fmrole lib_model_impl)); [| set_solver].
-      apply elem_of_subseteq. intros ? LIVE.
-      apply lib_model_impl_lr_strong in LIVE as [? [?]]. lia.
-    + apply ls_same_doms.
-    + done.
-  (* TODO: fix this weird error *)
-  (* Qed. *)
-  Admitted.
+(*   (* TODO: move to library, weaken Σ requirement *) *)
+(*   Lemma lib_premise_dis (lb: lm_ls lib_model) *)
+(*     (LB_INFO: lib_ls_premise lb): *)
+(*     ρlg ∈ live_roles lib_fair lb. *)
+(*   Proof.  *)
+(*     apply LM_live_roles_strong. *)
+(*     destruct LB_INFO as (F & S & TM). *)
+(*     eset (δ := ({| ls_under := (0: fmstate lib_model_impl); ls_fuel := ls_fuel lb; ls_mapping := ls_mapping lb; ls_inv := _ |})).      *)
+(*     exists δ. red. exists (Take_step ρl ρlg). split; [| done].     *)
+(*     repeat split; eauto. *)
+(*     - eapply ls_mapping_tmap_corr. eexists. split; eauto. set_solver. *)
+(*     - red. intros. inversion H2; subst; try set_solver. *)
+(*       destruct ρ', ρl; done. *)
+(*     - red. intros. left. *)
+(*       replace ρ' with ρl by (by destruct ρ', ρl).  *)
+(*       rewrite F. simpl. lia. *)
+(*     - intros. rewrite F. simpl. lia. *)
+(*     - intros. subst δ. simpl in H0. set_solver. *)
+(*     - subst δ. simpl. set_solver. *)
+(*     Unshelve. *)
+(*     + simpl. transitivity (∅: gset (fmrole lib_model_impl)); [| set_solver]. *)
+(*       apply elem_of_subseteq. intros ? LIVE. *)
+(*       apply lib_model_impl_lr_strong in LIVE as [? [?]]. lia. *)
+(*     + apply ls_same_doms. *)
+(*     + done. *)
+(*   (* TODO: fix this weird error *) *)
+(*   (* Qed. *) *)
+(*   Admitted. *)
       
     
 
-  (* TODO: move to library, weaken Σ requirement *)
-  Lemma lib_premise `{clientGS Σ} (lb: lm_ls lib_model)
-    (LB_INFO: lib_ls_premise lb):
-    ⊢ (frag_model_is (ls_under lb) -∗ frag_fuel_is (ls_fuel lb) -∗ frag_mapping_is (ls_tmap lb) -∗
-    frag_model_is (1: fmstate lib_model_impl) ∗ frag_mapping_is {[ρlg := {[ρl]}]} ∗ frag_fuel_is {[ρl := 2]})%I.
-  Proof. 
-    iIntros "LST LF LM".
-    destruct LB_INFO as (LIBF & -> & LIBM).
-    iFrame "LST". iSplitL "LM".
-    { rewrite -frag_mapping_is_big_sepM. 
-      2: { intros E. by rewrite E in LIBM. }
-      erewrite big_opM_insert_delete'; eauto.
-      iDestruct "LM" as "[??]". iFrame. }
-    rewrite -frag_fuel_is_big_sepM.
-    2: { intros E. by rewrite E in LIBF. }
-    erewrite big_opM_insert_delete'; eauto.
-    iDestruct "LF" as "[??]". iFrame. 
-  Qed.
+(*   (* TODO: move to library, weaken Σ requirement *) *)
+(*   Lemma lib_premise `{clientGS Σ} (lb: lm_ls lib_model) *)
+(*     (LB_INFO: lib_ls_premise lb): *)
+(*     ⊢ (frag_model_is (ls_under lb) -∗ frag_fuel_is (ls_fuel lb) -∗ frag_mapping_is (ls_tmap lb) -∗ *)
+(*     frag_model_is (1: fmstate lib_model_impl) ∗ frag_mapping_is {[ρlg := {[ρl]}]} ∗ frag_fuel_is {[ρl := 2]})%I. *)
+(*   Proof.  *)
+(*     iIntros "LST LF LM". *)
+(*     destruct LB_INFO as (LIBF & -> & LIBM). *)
+(*     iFrame "LST". iSplitL "LM". *)
+(*     { rewrite -frag_mapping_is_big_sepM.  *)
+(*       2: { intros E. by rewrite E in LIBM. } *)
+(*       erewrite big_opM_insert_delete'; eauto. *)
+(*       iDestruct "LM" as "[??]". iFrame. } *)
+(*     rewrite -frag_fuel_is_big_sepM. *)
+(*     2: { intros E. by rewrite E in LIBF. } *)
+(*     erewrite big_opM_insert_delete'; eauto. *)
+(*     iDestruct "LF" as "[??]". iFrame.  *)
+(*   Qed. *)
 
-  Lemma init_client_inv lb0 n:
-    partial_model_is (lb0, n)  ={∅}=∗ 
-    ∃ (cG: clientGS Σ), client_inv ∗
-                        frag_fuel_is (ls_fuel lb0) (fG := cl_lib_Σ) ∗
-                        frag_mapping_is (ls_tmap lb0 (LM := lib_model)) (fG := cl_lib_Σ)∗
-                        frag_model_is lb0 (fG := cl_lib_Σ)∗
-                        frag_free_roles_are ∅ (fG := cl_lib_Σ)∗
-                        y_frag_model_is n.
-  Proof using cpG.
-    iIntros "ST".
+(*   Lemma init_client_inv lb0 n: *)
+(*     partial_model_is (lb0, n)  ={∅}=∗  *)
+(*     ∃ (cG: clientGS Σ), client_inv ∗ *)
+(*                         frag_fuel_is (ls_fuel lb0) (fG := cl_lib_Σ) ∗ *)
+(*                         frag_mapping_is (ls_tmap lb0 (LM := lib_model)) (fG := cl_lib_Σ)∗ *)
+(*                         frag_model_is lb0 (fG := cl_lib_Σ)∗ *)
+(*                         frag_free_roles_are ∅ (fG := cl_lib_Σ)∗ *)
+(*                         y_frag_model_is n. *)
+(*   Proof using cpG. *)
+(*     iIntros "ST". *)
         
-    iMod (lm_msi_init lb0 ∅) as (fG) "(MSI_LIB & FRAG_LIB & FRAG_MAP & FRAG_FUEL & FRAG_FR)".
-    { set_solver. }
+(*     iMod (lm_msi_init lb0 ∅) as (fG) "(MSI_LIB & FRAG_LIB & FRAG_MAP & FRAG_FUEL & FRAG_FR)". *)
+(*     { set_solver. } *)
 
-    iMod (own_alloc ((● (Excl' n) ⋅ ◯ _))) as (γ_st) "[AUTH_Y FRAG_Y]".
-    { apply auth_both_valid_discrete. split; [| done]. reflexivity. }
+(*     iMod (own_alloc ((● (Excl' n) ⋅ ◯ _))) as (γ_st) "[AUTH_Y FRAG_Y]". *)
+(*     { apply auth_both_valid_discrete. split; [| done]. reflexivity. } *)
 
-    set (cG := {| 
-                cl_pre_inG := cpG;
-                cl_y_st_name := γ_st;
-                cl_lib_Σ := fG;
-              |}). 
+(*     set (cG := {|  *)
+(*                 cl_pre_inG := cpG; *)
+(*                 cl_y_st_name := γ_st; *)
+(*                 cl_lib_Σ := fG; *)
+(*               |}).  *)
  
-    iMod (inv_alloc Ns _  (∃ st, client_inv_impl st) with "[-FRAG_LIB FRAG_Y FRAG_MAP FRAG_FR FRAG_FUEL]") as "#INV".
-    { iNext. rewrite /client_inv_impl. 
-      iExists (_, _). iFrame. }
+(*     iMod (inv_alloc Ns _  (∃ st, client_inv_impl st) with "[-FRAG_LIB FRAG_Y FRAG_MAP FRAG_FR FRAG_FUEL]") as "#INV". *)
+(*     { iNext. rewrite /client_inv_impl.  *)
+(*       iExists (_, _). iFrame. } *)
 
-    iModIntro. iExists _. iFrame. done. 
-  Qed.
+(*     iModIntro. iExists _. iFrame. done.  *)
+(*   Qed. *)
 
-  Lemma live_roles_1 lb:
-    live_roles client_model_impl (lb, 1) = 
-    if (decide (ρlg ∈ live_roles _ lb)) 
-    then {[ inl ρlg ]} 
-    else if decide (ls_tmap lb (LM := lib_model) !! ρlg = Some ∅) 
-         then {[ inr ρy ]} 
-         else ∅. 
-  Proof. 
-    simpl. rewrite /client_lr.
-    apply leibniz_equiv. rewrite filter_union.
+(*   Lemma live_roles_1 lb: *)
+(*     live_roles client_model_impl (lb, 1) =  *)
+(*     if (decide (ρlg ∈ live_roles _ lb))  *)
+(*     then {[ inl ρlg ]}  *)
+(*     else if decide (ls_tmap lb (LM := lib_model) !! ρlg = Some ∅)  *)
+(*          then {[ inr ρy ]}  *)
+(*          else ∅.  *)
+(*   Proof.  *)
+(*     simpl. rewrite /client_lr. *)
+(*     apply leibniz_equiv. rewrite filter_union. *)
 
-    destruct (decide (ρlg ∈ live_roles lib_fair lb)) as [LR | LR].
-    - pose proof (LM_live_role_map_notempty _ _ LR) as (?&MAP&?).
-      erewrite filter_singleton, filter_singleton_not, decide_True.
-      + set_solver.
-      + eauto.
-      + rewrite bool_decide_eq_false_2; [done| ].
-        intros [? STEP]. inversion STEP. subst. set_solver.
-      + rewrite bool_decide_eq_true_2; [done| ].
-        eapply LM_live_roles_strong in LR as [? ?]. eauto. 
-        eexists. eapply ct_lib_step. simpl. eauto.
-    - rewrite filter_singleton_not; [rewrite decide_False| ]. 
-      2: { intros [DOM LIVE]%elem_of_filter.
-           by apply LM_live_roles_strong in DOM. }
-      2: { rewrite bool_decide_eq_false_2; [done| ].
-           intros [? STEP]. inversion STEP. subst. simpl in LIB_STEP.
-           destruct LR. apply LM_live_roles_strong. eauto. }
-      destruct (ls_tmap lb (LM := lib_model) !! ρlg) eqn:MAP0.
-      (* ; rewrite MAP0. *)
-      + destruct (decide (g = ∅)) as [-> | ?]. 
-        * erewrite decide_True; [| done].
-          rewrite filter_singleton; [set_solver| ].
-          rewrite bool_decide_eq_true_2; [done| ]. eexists. by econstructor.
-        * erewrite decide_False.
-          2: { intros [=]. done. }
-          rewrite filter_singleton_not; [set_solver| ].
-          rewrite bool_decide_eq_false_2; [done| ].
-          intros [? STEP]. inversion STEP. subst.
-          rewrite MAP0 in LIB_NOROLES. congruence.
-      + erewrite decide_False; [| done].
-        rewrite filter_singleton_not; [set_solver| ].
-        rewrite bool_decide_eq_false_2; [done| ].
-        intros [? STEP]. inversion STEP. subst.
-        rewrite MAP0 in LIB_NOROLES. congruence.
-  Qed. 
+(*     destruct (decide (ρlg ∈ live_roles lib_fair lb)) as [LR | LR]. *)
+(*     - pose proof (LM_live_role_map_notempty _ _ LR) as (?&MAP&?). *)
+(*       erewrite filter_singleton, filter_singleton_not, decide_True. *)
+(*       + set_solver. *)
+(*       + eauto. *)
+(*       + rewrite bool_decide_eq_false_2; [done| ]. *)
+(*         intros [? STEP]. inversion STEP. subst. set_solver. *)
+(*       + rewrite bool_decide_eq_true_2; [done| ]. *)
+(*         eapply LM_live_roles_strong in LR as [? ?]. eauto.  *)
+(*         eexists. eapply ct_lib_step. simpl. eauto. *)
+(*     - rewrite filter_singleton_not; [rewrite decide_False| ].  *)
+(*       2: { intros [DOM LIVE]%elem_of_filter. *)
+(*            by apply LM_live_roles_strong in DOM. } *)
+(*       2: { rewrite bool_decide_eq_false_2; [done| ]. *)
+(*            intros [? STEP]. inversion STEP. subst. simpl in LIB_STEP. *)
+(*            destruct LR. apply LM_live_roles_strong. eauto. } *)
+(*       destruct (ls_tmap lb (LM := lib_model) !! ρlg) eqn:MAP0. *)
+(*       (* ; rewrite MAP0. *) *)
+(*       + destruct (decide (g = ∅)) as [-> | ?].  *)
+(*         * erewrite decide_True; [| done]. *)
+(*           rewrite filter_singleton; [set_solver| ]. *)
+(*           rewrite bool_decide_eq_true_2; [done| ]. eexists. by econstructor. *)
+(*         * erewrite decide_False. *)
+(*           2: { intros [=]. done. } *)
+(*           rewrite filter_singleton_not; [set_solver| ]. *)
+(*           rewrite bool_decide_eq_false_2; [done| ]. *)
+(*           intros [? STEP]. inversion STEP. subst. *)
+(*           rewrite MAP0 in LIB_NOROLES. congruence. *)
+(*       + erewrite decide_False; [| done]. *)
+(*         rewrite filter_singleton_not; [set_solver| ]. *)
+(*         rewrite bool_decide_eq_false_2; [done| ]. *)
+(*         intros [? STEP]. inversion STEP. subst. *)
+(*         rewrite MAP0 in LIB_NOROLES. congruence. *)
+(*   Qed.  *)
 
-  Lemma live_roles_2 lb0:
-    live_roles client_model_impl (lb0, 2) ≡ {[ inr ρy ]}.
-  Proof. 
-    simpl. rewrite /client_lr.
-    rewrite filter_union.
-    erewrite filter_singleton_not, filter_singleton; [set_solver| ..].
-    - rewrite bool_decide_eq_true_2; [done| ]. eexists. econstructor.
-    - apply not_true_iff_false. 
-      rewrite bool_decide_eq_false_2; [tauto| ].
-      intros [? STEP]. inversion STEP.
-  Qed. 
+(*   Lemma live_roles_2 lb0: *)
+(*     live_roles client_model_impl (lb0, 2) ≡ {[ inr ρy ]}. *)
+(*   Proof.  *)
+(*     simpl. rewrite /client_lr. *)
+(*     rewrite filter_union. *)
+(*     erewrite filter_singleton_not, filter_singleton; [set_solver| ..]. *)
+(*     - rewrite bool_decide_eq_true_2; [done| ]. eexists. econstructor. *)
+(*     - apply not_true_iff_false.  *)
+(*       rewrite bool_decide_eq_false_2; [tauto| ]. *)
+(*       intros [? STEP]. inversion STEP. *)
+(*   Qed.  *)
 
-  Lemma live_roles_0 lb:
-    live_roles client_model_impl (lb, 0) = ∅.
-  Proof. 
-    simpl. rewrite /client_lr.
-    apply leibniz_equiv. rewrite filter_union.
-    erewrite !filter_singleton_not; [set_solver| ..].
-    all: rewrite bool_decide_eq_false_2; [done| ].
-    all: intros [? STEP]; inversion STEP.
-  Qed. 
+(*   Lemma live_roles_0 lb: *)
+(*     live_roles client_model_impl (lb, 0) = ∅. *)
+(*   Proof.  *)
+(*     simpl. rewrite /client_lr. *)
+(*     apply leibniz_equiv. rewrite filter_union. *)
+(*     erewrite !filter_singleton_not; [set_solver| ..]. *)
+(*     all: rewrite bool_decide_eq_false_2; [done| ]. *)
+(*     all: intros [? STEP]; inversion STEP. *)
+(*   Qed.  *)
 
-  Tactic Notation "specialize_full" ident(H) :=
-    let foo := fresh in
-    evar (foo : Prop); cut (foo); subst foo; cycle 1; [eapply H|try clear H; intro H].
+(*   Tactic Notation "specialize_full" ident(H) := *)
+(*     let foo := fresh in *)
+(*     evar (foo : Prop); cut (foo); subst foo; cycle 1; [eapply H|try clear H; intro H]. *)
 
 
-  (* TODO: make it a library LSI *)
-  Lemma lib_tmap_dom_restricted (δ: fmstate lib_fair):
-    dom (ls_tmap δ (LM := lib_model)) ⊆ {[ ρlg ]}.
-  Proof. Admitted.
+(*   (* TODO: make it a library LSI *) *)
+(*   Lemma lib_tmap_dom_restricted (δ: fmstate lib_fair): *)
+(*     dom (ls_tmap δ (LM := lib_model)) ⊆ {[ ρlg ]}. *)
+(*   Proof. Admitted. *)
 
-  Lemma update_client_state `{clientGS Σ} Einvs
-    (extr: execution_trace heap_lang) (mtr: auxiliary_trace M)
-    c2 (lb lb': fmstate lib_fair) f
-    (LIB_STEP: locale_trans lb ρlg lb' (LM := lib_model))
-    (PROG_STEP: locale_step (trace_last extr) (Some 0) c2)
-    (F_BOUND: f ≤ client_fl)
-    :
-    LSG Einvs ⊢
-    em_msi (trace_last extr) (trace_last mtr) (em_GS0 := heap_fairnessGS) -∗ 
-    partial_model_is (lb, 1) -∗
-    partial_free_roles_are {[inr ρy]} -∗
-    has_fuels 0 {[inl ρlg := f]}
-    ={Einvs}=∗
-    ∃ (δ2 : M) (ℓ: mlabel M),
-      ⌜em_valid_evolution_step (Some 0) c2 (trace_last mtr) ℓ δ2⌝ ∗
-      em_msi c2 δ2 (em_GS0 := heap_fairnessGS) ∗
-      has_fuels 0 (if decide (ls_tmap lb' (LM := lib_model) !! ρlg = Some ∅)
-                   then {[inr ρy := client_fl]}
-                   else {[inl ρlg := f]}) ∗
-      partial_model_is (lb', 1) ∗
-      partial_free_roles_are
-      (if decide (ls_tmap lb' (LM := lib_model) !! ρlg = Some ∅) then {[inl ρlg]} else {[inr ρy]}).
-  Proof.
+(*   Lemma update_client_state `{clientGS Σ} Einvs *)
+(*     (extr: execution_trace heap_lang) (mtr: auxiliary_trace M) *)
+(*     c2 (lb lb': fmstate lib_fair) f *)
+(*     (LIB_STEP: locale_trans lb ρlg lb' (LM := lib_model)) *)
+(*     (PROG_STEP: locale_step (trace_last extr) (Some 0) c2) *)
+(*     (F_BOUND: f ≤ client_fl) *)
+(*     : *)
+(*     LSG Einvs ⊢ *)
+(*     em_msi (trace_last extr) (trace_last mtr) (em_GS0 := heap_fairnessGS) -∗  *)
+(*     partial_model_is (lb, 1) -∗ *)
+(*     partial_free_roles_are {[inr ρy]} -∗ *)
+(*     has_fuels 0 {[inl ρlg := f]} *)
+(*     ={Einvs}=∗ *)
+(*     ∃ (δ2 : M) (ℓ: mlabel M), *)
+(*       ⌜em_valid_evolution_step (Some 0) c2 (trace_last mtr) ℓ δ2⌝ ∗ *)
+(*       em_msi c2 δ2 (em_GS0 := heap_fairnessGS) ∗ *)
+(*       has_fuels 0 (if decide (ls_tmap lb' (LM := lib_model) !! ρlg = Some ∅) *)
+(*                    then {[inr ρy := client_fl]} *)
+(*                    else {[inl ρlg := f]}) ∗ *)
+(*       partial_model_is (lb', 1) ∗ *)
+(*       partial_free_roles_are *)
+(*       (if decide (ls_tmap lb' (LM := lib_model) !! ρlg = Some ∅) then {[inl ρlg]} else {[inr ρy]}). *)
+(*   Proof. *)
     
-    iIntros "#PMP MSI ST FR FUELS".
-    Local Ltac dEq := destruct (decide (_ = _)). 
-    Local Ltac dEl := destruct (decide (_ ∈ _)). 
-    pose proof (LM_map_empty_notlive lb' ρlg (LM := lib_model) (INH_LM := lib_model_inh)).
+(*     iIntros "#PMP MSI ST FR FUELS". *)
+(*     Local Ltac dEq := destruct (decide (_ = _)).  *)
+(*     Local Ltac dEl := destruct (decide (_ ∈ _)).  *)
+(*     pose proof (LM_map_empty_notlive lb' ρlg (LM := lib_model)). *)
 
-    pose proof (live_roles_1 lb) as LIVE. rewrite decide_True in LIVE. 
-    2: { eapply LM_live_roles_strong. eexists. eauto. }
-    (* TODO: consider the case with rem ≠ ∅ *)
-    pose proof (live_roles_1 lb') as LIVE'.
+(*     pose proof (live_roles_1 lb) as LIVE. rewrite decide_True in LIVE.  *)
+(*     2: { eapply LM_live_roles_strong. eexists. eauto. } *)
+(*     (* TODO: consider the case with rem ≠ ∅ *) *)
+(*     pose proof (live_roles_1 lb') as LIVE'. *)
 
-    remember (trace_last extr) as c1. destruct c1 as (σ1, tp1).
-    destruct c2 as (σ2, tp2).
+(*     remember (trace_last extr) as c1. destruct c1 as (σ1, tp1). *)
+(*     destruct c2 as (σ2, tp2). *)
 
-    iPoseProof (update_step_still_alive_gen with "[$] [$] [$] [$] [$]") as "EM_STEP".
-    7: { apply PROG_STEP. }
-    7: { apply ct_lib_step. simpl. eauto. }
-    { rewrite LIVE LIVE'.
-      apply union_subseteq_l'. 
-      dEl; set_solver. }
-    { rewrite dom_singleton.
-      assert ((if (decide (ls_tmap lb' (LM := lib_model) !! ρlg = Some ∅))
-              then {[ inl ρlg ]}
-              else (∅: gset (fmrole client_model_impl))) ⊆ {[inl ρlg]}) as IN.
-      { dEq; set_solver. }
-      apply IN. }
-    { rewrite LIVE. set_solver. }
-    all: eauto.
-    { Unshelve.
-      2: exact (if decide (ls_tmap lb' (LM := lib_model) !! ρlg = Some ∅)
-                then {[ inr ρy := client_fl ]}
-                else {[ inl ρlg := f ]}).
-      destruct (decide (_=_)); set_solver. }
-    { repeat split; rewrite ?LIVE ?LIVE'.
-      - dEl.
-        2: { destruct decide; set_solver. }
-        intros _. rewrite decide_False.
-        { rewrite lookup_singleton. simpl. lia. }
-        tauto.
-      - destruct (decide (_ ∈ _)); [set_solver| ].
-        destruct (decide (_=_)); [set_solver| ].
-        rewrite !lookup_singleton. simpl. lia.
-      - set_solver.
-      - dEq; [| set_solver].
-        intros. assert (ρ' = inr ρy) as -> by set_solver.
-        rewrite lookup_singleton. simpl. lia.
-      - dEq; set_solver.
-      - dEq; dEl; set_solver.
-      - dEq; dEl; set_solver. }
-    { red. intros. red.
-      (* TODO: move this simplification, as it occurs quite often *)
-      rewrite /update_mapping. rewrite map_imap_dom_eq.
-      2: { rewrite dom_gset_to_gmap. intro.
-           destruct (decide (k ∈ dom R)); [| done].
-           intros. by eapply elem_of_dom. }
-      rewrite dom_gset_to_gmap. intros g' IN'.
-      red in H2.
-      (* at this point we must ensure that no new group roles 
-         were created by a lib step *)
+(*     iPoseProof (update_step_still_alive_gen with "[$] [$] [$] [$] [$]") as "EM_STEP". *)
+(*     7: { apply PROG_STEP. } *)
+(*     7: { apply ct_lib_step. simpl. eauto. } *)
+(*     { rewrite LIVE LIVE'. *)
+(*       apply union_subseteq_l'.  *)
+(*       dEl; set_solver. } *)
+(*     { rewrite dom_singleton. *)
+(*       assert ((if (decide (ls_tmap lb' (LM := lib_model) !! ρlg = Some ∅)) *)
+(*               then {[ inl ρlg ]} *)
+(*               else (∅: gset (fmrole client_model_impl))) ⊆ {[inl ρlg]}) as IN. *)
+(*       { dEq; set_solver. } *)
+(*       apply IN. } *)
+(*     { rewrite LIVE. set_solver. } *)
+(*     all: eauto. *)
+(*     { Unshelve. *)
+(*       2: exact (if decide (ls_tmap lb' (LM := lib_model) !! ρlg = Some ∅) *)
+(*                 then {[ inr ρy := client_fl ]} *)
+(*                 else {[ inl ρlg := f ]}). *)
+(*       destruct (decide (_=_)); set_solver. } *)
+(*     { repeat split; rewrite ?LIVE ?LIVE'. *)
+(*       - dEl. *)
+(*         2: { destruct decide; set_solver. } *)
+(*         intros _. rewrite decide_False. *)
+(*         { rewrite lookup_singleton. simpl. lia. } *)
+(*         tauto. *)
+(*       - destruct (decide (_ ∈ _)); [set_solver| ]. *)
+(*         destruct (decide (_=_)); [set_solver| ]. *)
+(*         rewrite !lookup_singleton. simpl. lia. *)
+(*       - set_solver. *)
+(*       - dEq; [| set_solver]. *)
+(*         intros. assert (ρ' = inr ρy) as -> by set_solver. *)
+(*         rewrite lookup_singleton. simpl. lia. *)
+(*       - dEq; set_solver. *)
+(*       - dEq; dEl; set_solver. *)
+(*       - dEq; dEl; set_solver. } *)
+(*     { red. intros. red. *)
+(*       (* TODO: move this simplification, as it occurs quite often *) *)
+(*       rewrite /update_mapping. rewrite map_imap_dom_eq. *)
+(*       2: { rewrite dom_gset_to_gmap. intro. *)
+(*            destruct (decide (k ∈ dom R)); [| done]. *)
+(*            intros. by eapply elem_of_dom. } *)
+(*       rewrite dom_gset_to_gmap. intros g' IN'. *)
+(*       red in H2. *)
+(*       (* at this point we must ensure that no new group roles  *)
+(*          were created by a lib step *) *)
 
-      destruct IN' as [? IN']. simpl in IN'.
-      apply (ls_mapping_tmap_corr (LM := lib_model)) in IN' as (?&?&?).
-      pose proof (lib_tmap_dom_restricted lb') as DOML.
-      specialize (DOML g'). specialize_full DOML.
-      { apply elem_of_dom. set_solver. }
-      apply elem_of_singleton_1 in DOML. subst g'.
-      rewrite decide_False; [set_solver| ].
-      intros EMP. set_solver. }
+(*       destruct IN' as [? IN']. simpl in IN'. *)
+(*       apply (ls_mapping_tmap_corr (LM := lib_model)) in IN' as (?&?&?). *)
+(*       pose proof (lib_tmap_dom_restricted lb') as DOML. *)
+(*       specialize (DOML g'). specialize_full DOML. *)
+(*       { apply elem_of_dom. set_solver. } *)
+(*       apply elem_of_singleton_1 in DOML. subst g'. *)
+(*       rewrite decide_False; [set_solver| ]. *)
+(*       intros EMP. set_solver. } *)
       
-    rewrite LIVE LIVE'.
-    iMod "EM_STEP" as (??) "(?&?&?&?&FREE)".
-    iModIntro. do 2 iExists _. iFrame.
+(*     rewrite LIVE LIVE'. *)
+(*     iMod "EM_STEP" as (??) "(?&?&?&?&FREE)". *)
+(*     iModIntro. do 2 iExists _. iFrame. *)
     
-    iApply partial_free_roles_are_Proper; [| iFrame].
-    dEl; dEq; tauto || set_solver.
-  Qed. 
+(*     iApply partial_free_roles_are_Proper; [| iFrame]. *)
+(*     dEl; dEq; tauto || set_solver. *)
+(*   Qed.  *)
 
-  (* TODO: unify with model_agree ? *)
-  Lemma y_model_agree `{clientGS Σ} y1 y2:
-    ⊢ y_auth_model_is y1 -∗ y_frag_model_is y2 -∗ ⌜y1 = y2⌝.
-  Proof. 
-    iIntros "Ha Hf".
-    by iDestruct (own_valid_2 with "Ha Hf") as
-      %[Heq%Excl_included%leibniz_equiv ?]%auth_both_valid_discrete.
-  Qed.
+(*   (* TODO: unify with model_agree ? *) *)
+(*   Lemma y_model_agree `{clientGS Σ} y1 y2: *)
+(*     ⊢ y_auth_model_is y1 -∗ y_frag_model_is y2 -∗ ⌜y1 = y2⌝. *)
+(*   Proof.  *)
+(*     iIntros "Ha Hf". *)
+(*     by iDestruct (own_valid_2 with "Ha Hf") as *)
+(*       %[Heq%Excl_included%leibniz_equiv ?]%auth_both_valid_discrete. *)
+(*   Qed. *)
 
-  (* TODO: unify with update_model ? *)
-  Lemma y_update_model `{clientGS Σ} y1 y2 y:
-    y_auth_model_is y1 -∗ y_frag_model_is y2 ==∗ y_auth_model_is y ∗ y_frag_model_is y.
-  Proof.
-    iIntros "H1 H2". iCombine "H1 H2" as "H".
-    iMod (own_update with "H") as "[??]" ; eauto.
-    - by apply auth_update, option_local_update, (exclusive_local_update _ (Excl y)).
-    - iModIntro. iFrame.
-  Qed.
+(*   (* TODO: unify with update_model ? *) *)
+(*   Lemma y_update_model `{clientGS Σ} y1 y2 y: *)
+(*     y_auth_model_is y1 -∗ y_frag_model_is y2 ==∗ y_auth_model_is y ∗ y_frag_model_is y. *)
+(*   Proof. *)
+(*     iIntros "H1 H2". iCombine "H1 H2" as "H". *)
+(*     iMod (own_update with "H") as "[??]" ; eauto. *)
+(*     - by apply auth_update, option_local_update, (exclusive_local_update _ (Excl y)). *)
+(*     - iModIntro. iFrame. *)
+(*   Qed. *)
      
-(*   Lemma big_opM_fmap': *)
-(*   ∀ {M M' : ofe} {o : M → M → M} {o' : M' → M' → M'} *)
-(*     {Monoid0 : Monoid o} {Monoid0' : Monoid o'} {K : Type} *)
-(*     {EqDecision0 : EqDecision K} {H : Countable K} *)
-(*     (f : M → M') (m : gmap K M), *)
-(*     (([^ op map] k↦y ∈ m, f <$> ({[ k := y ]}: gmap K M)): gmap K M') = (f <$> m: gmap K M'). *)
-(* (* f <$> {[k := ]} *) *)
+(* (*   Lemma big_opM_fmap': *) *)
+(* (*   ∀ {M M' : ofe} {o : M → M → M} {o' : M' → M' → M'} *) *)
+(* (*     {Monoid0 : Monoid o} {Monoid0' : Monoid o'} {K : Type} *) *)
+(* (*     {EqDecision0 : EqDecision K} {H : Countable K} *) *)
+(* (*     (f : M → M') (m : gmap K M), *) *)
+(* (*     (([^ op map] k↦y ∈ m, f <$> ({[ k := y ]}: gmap K M)): gmap K M') = (f <$> m: gmap K M'). *) *)
+(* (* (* f <$> {[k := ]} *) *) *)
 
 
-  Lemma lib_open_inv `{clientGS Σ} ζ fs (FSnz : fs ≠ ∅):
-    client_inv -∗ has_fuels ζ fs (PMPP := lib_PMPP) -∗
-    |={↑Ns, ∅}=>
-    ⌜ ζ = 0 ⌝ ∗
-    (∃ lb, partial_model_is (lb, 1) (PartialModelPredicatesPre := PMPP) ∗ model_state_interp lb) ∗ 
-    frag_mapping_is {[ρlg := dom fs]}  ∗ y_auth_model_is 1 ∗
-    (∃ f, partial_fuel_is {[inl ρlg := f]} ∗ ⌜ 1 <= f <= client_fl ⌝) ∗
-    partial_mapping_is {[0 := {[inl ρlg]}]} ∗
-    partial_free_roles_are {[inr ρy]} ∗ y_frag_model_is 1 ∗
-    frag_fuel_is fs ∗
-    (▷ (∃ st, client_inv_impl st) ={ ∅, ↑Ns}=∗ emp).
-  Proof.
-    iIntros "#INV FUELS_LIB".
-    iInv Ns as ((lb, y)) ">(ST & YST_AUTH & inv')" "CLOS".
-    rewrite difference_diag_L. iModIntro.  
-    iDestruct (has_fuels_equiv with "FUELS_LIB") as "[MAP_LIB FUEL_LIB]". 
-    simpl. iDestruct "MAP_LIB" as (???) "(%LIBM&LM&MATCH&MAP&FR&YST)". 
-    assert (ζ = 0 /\ L = dom fs) as [-> ->]; [| clear LIBM].
-    { by apply map_singleton_inj in LIBM as [-> <-]. }
-    (* assert (S <$> fs ≠ ∅) by (by intros ?%fmap_empty_inv). *)
-    iDestruct "MATCH" as "[(_&[-> ->]&(%f & Ff & %BOUND)) | [% _]]".
-    2: { exfalso. apply FSnz. apply dom_empty_iff. set_solver. }
-    iPoseProof (y_model_agree with "YST_AUTH YST") as "->".
-    iPoseProof (frag_mapping_same with "[inv'] LM") as "%TMAP0".
-    { iDestruct "inv'" as (?)"(?&?&?)". iFrame. }
-    iPoseProof (frag_fuel_included with "[inv'] [FUEL_LIB]") as "%FUEL0".
-    { iDestruct "inv'" as (?)"(?&?&?&?)". iFrame. }
-    { iApply frag_fuel_is_big_sepM; [done | by iFrame]. }
-    iSplitR; [done| ]. 
-    iFrame. iSplitL "ST inv'".
-    - iExists _. iFrame.
-    - iDestruct (frag_fuel_is_big_sepM with "FUEL_LIB") as "?"; [done| ].
-      iFrame. iExists _. iFrame. done. 
-  Qed.
+(*   Lemma lib_open_inv `{clientGS Σ} ζ fs (FSnz : fs ≠ ∅): *)
+(*     client_inv -∗ has_fuels ζ fs (PMPP := lib_PMPP) -∗ *)
+(*     |={↑Ns, ∅}=> *)
+(*     ⌜ ζ = 0 ⌝ ∗ *)
+(*     (∃ lb, partial_model_is (lb, 1) (PartialModelPredicatesPre := PMPP) ∗ model_state_interp lb) ∗  *)
+(*     frag_mapping_is {[ρlg := dom fs]}  ∗ y_auth_model_is 1 ∗ *)
+(*     (∃ f, partial_fuel_is {[inl ρlg := f]} ∗ ⌜ 1 <= f <= client_fl ⌝) ∗ *)
+(*     partial_mapping_is {[0 := {[inl ρlg]}]} ∗ *)
+(*     partial_free_roles_are {[inr ρy]} ∗ y_frag_model_is 1 ∗ *)
+(*     frag_fuel_is fs ∗ *)
+(*     (▷ (∃ st, client_inv_impl st) ={ ∅, ↑Ns}=∗ emp). *)
+(*   Proof. *)
+(*     iIntros "#INV FUELS_LIB". *)
+(*     iInv Ns as ((lb, y)) ">(ST & YST_AUTH & inv')" "CLOS". *)
+(*     rewrite difference_diag_L. iModIntro.   *)
+(*     iDestruct (has_fuels_equiv with "FUELS_LIB") as "[MAP_LIB FUEL_LIB]".  *)
+(*     simpl. iDestruct "MAP_LIB" as (???) "(%LIBM&LM&MATCH&MAP&FR&YST)".  *)
+(*     assert (ζ = 0 /\ L = dom fs) as [-> ->]; [| clear LIBM]. *)
+(*     { by apply map_singleton_inj in LIBM as [-> <-]. } *)
+(*     (* assert (S <$> fs ≠ ∅) by (by intros ?%fmap_empty_inv). *) *)
+(*     iDestruct "MATCH" as "[(_&[-> ->]&(%f & Ff & %BOUND)) | [% _]]". *)
+(*     2: { exfalso. apply FSnz. apply dom_empty_iff. set_solver. } *)
+(*     iPoseProof (y_model_agree with "YST_AUTH YST") as "->". *)
+(*     iPoseProof (frag_mapping_same with "[inv'] LM") as "%TMAP0". *)
+(*     { iDestruct "inv'" as (?)"(?&?&?)". iFrame. } *)
+(*     iPoseProof (frag_fuel_included with "[inv'] [FUEL_LIB]") as "%FUEL0". *)
+(*     { iDestruct "inv'" as (?)"(?&?&?&?)". iFrame. } *)
+(*     { iApply frag_fuel_is_big_sepM; [done | by iFrame]. } *)
+(*     iSplitR; [done| ].  *)
+(*     iFrame. iSplitL "ST inv'". *)
+(*     - iExists _. iFrame. *)
+(*     - iDestruct (frag_fuel_is_big_sepM with "FUEL_LIB") as "?"; [done| ]. *)
+(*       iFrame. iExists _. iFrame. done.  *)
+(*   Qed. *)
 
 
-  Lemma fuel_step_lifting `{clientGS Σ} Einvs (DISJ_INV: Einvs ## ↑Ns):
-  LSG Einvs ∗ client_inv ⊢
-  ∀ (extr : execution_trace heap_lang) (auxtr : auxiliary_trace M) 
-    (c2 : cfg heap_lang) (fs : gmap (fmrole lib_model_impl) nat) 
-    (ζ : locale heap_lang) (_ : dom fs ≠ ∅) (_ : locale_step 
-                                                   (trace_last extr) 
-                                                   (Some ζ) c2),
-    has_fuels ζ (S <$> fs) (PMPP := lib_PMPP) -∗
-    em_msi (trace_last extr) (trace_last auxtr) (em_GS0 := heap_fairnessGS)
-    ={Einvs ∪ ↑Ns}=∗
-    ∃ (δ2 : M) (ℓ : mlabel M),
-      ⌜em_valid_state_evolution_fairness (extr :tr[ Some ζ ]: c2)
-         (auxtr :tr[ ℓ ]: δ2)⌝ ∗
-      has_fuels ζ (filter (λ '(k, _), k ∈ dom fs ∖ ∅) fs) (PMPP := lib_PMPP) ∗ 
-      em_msi c2 δ2 (em_GS0 := heap_fairnessGS).
-  Proof.
-    iIntros "[#PMP #COMP]". iIntros "* FUELS_LIB MSI". simpl in *.
+(*   Lemma fuel_step_lifting `{clientGS Σ} Einvs (DISJ_INV: Einvs ## ↑Ns): *)
+(*   LSG Einvs ∗ client_inv ⊢ *)
+(*   ∀ (extr : execution_trace heap_lang) (auxtr : auxiliary_trace M)  *)
+(*     (c2 : cfg heap_lang) (fs : gmap (fmrole lib_model_impl) nat)  *)
+(*     (ζ : locale heap_lang) (_ : dom fs ≠ ∅) (_ : locale_step  *)
+(*                                                    (trace_last extr)  *)
+(*                                                    (Some ζ) c2), *)
+(*     has_fuels ζ (S <$> fs) (PMPP := lib_PMPP) -∗ *)
+(*     em_msi (trace_last extr) (trace_last auxtr) (em_GS0 := heap_fairnessGS) *)
+(*     ={Einvs ∪ ↑Ns}=∗ *)
+(*     ∃ (δ2 : M) (ℓ : mlabel M), *)
+(*       ⌜em_valid_state_evolution_fairness (extr :tr[ Some ζ ]: c2) *)
+(*          (auxtr :tr[ ℓ ]: δ2)⌝ ∗ *)
+(*       has_fuels ζ (filter (λ '(k, _), k ∈ dom fs ∖ ∅) fs) (PMPP := lib_PMPP) ∗  *)
+(*       em_msi c2 δ2 (em_GS0 := heap_fairnessGS). *)
+(*   Proof. *)
+(*     iIntros "[#PMP #COMP]". iIntros "* FUELS_LIB MSI". simpl in *. *)
     
-    assert (S <$> fs ≠ ∅) as NE.
-    { intros ?%dom_empty_iff. set_solver. }
+(*     assert (S <$> fs ≠ ∅) as NE. *)
+(*     { intros ?%dom_empty_iff. set_solver. } *)
 
-    iPoseProof (lib_open_inv with "[$] FUELS_LIB") as "INV'"; [set_solver| ].
-    rewrite union_comm_L. 
-    iMod (fupd_mask_frame_r _ _ Einvs with "INV'") as 
-      "(-> & (%lb & ST & inv') & LM & YST_AUTH & (%f & Ff & %BOUND) & MAP & FR & YST & FUEL_LIB & CLOS)"; [set_solver| ].
+(*     iPoseProof (lib_open_inv with "[$] FUELS_LIB") as "INV'"; [set_solver| ]. *)
+(*     rewrite union_comm_L.  *)
+(*     iMod (fupd_mask_frame_r _ _ Einvs with "INV'") as  *)
+(*       "(-> & (%lb & ST & inv') & LM & YST_AUTH & (%f & Ff & %BOUND) & MAP & FR & YST & FUEL_LIB & CLOS)"; [set_solver| ]. *)
     
-    iMod (actual_update_no_step_enough_fuel with "[LM FUEL_LIB] inv'") as (lb') "(%LIB_STEP & FUELS_LIB & MSI_LIB & %TMAP_LIB)".
-    3: { apply empty_subseteq. }
-    { eauto. }
-    { set_solver. }
-    { rewrite /has_fuels_S. rewrite has_fuels_equiv. iFrame.      
-      iApply frag_fuel_is_big_sepM; done. }
+(*     iMod (actual_update_no_step_enough_fuel with "[LM FUEL_LIB] inv'") as (lb') "(%LIB_STEP & FUELS_LIB & MSI_LIB & %TMAP_LIB)". *)
+(*     3: { apply empty_subseteq. } *)
+(*     { eauto. } *)
+(*     { set_solver. } *)
+(*     { rewrite /has_fuels_S. rewrite has_fuels_equiv. iFrame.       *)
+(*       iApply frag_fuel_is_big_sepM; done. } *)
     
-    destruct (trace_last extr) as (σ1, tp1) eqn:LASTE. destruct c2 as (σ2, tp2).
-    rewrite LASTE. 
-    rewrite difference_empty_L. rewrite difference_empty_L in TMAP_LIB.
-    iAssert (has_fuels 0 {[ inl ρlg := f ]}) with "[MAP Ff]" as "FUELS".
-    { rewrite /has_fuels. rewrite dom_singleton_L big_sepS_singleton.
-      rewrite lookup_singleton. iFrame. iExists _. iFrame. done. }
+(*     destruct (trace_last extr) as (σ1, tp1) eqn:LASTE. destruct c2 as (σ2, tp2). *)
+(*     rewrite LASTE.  *)
+(*     rewrite difference_empty_L. rewrite difference_empty_L in TMAP_LIB. *)
+(*     iAssert (has_fuels 0 {[ inl ρlg := f ]}) with "[MAP Ff]" as "FUELS". *)
+(*     { rewrite /has_fuels. rewrite dom_singleton_L big_sepS_singleton. *)
+(*       rewrite lookup_singleton. iFrame. iExists _. iFrame. done. } *)
 
-    rewrite -LASTE. 
-    iPoseProof (update_client_state with "[$] [$] [$] [$] [$]") as "EM_STEP"; eauto.
-    { eexists. split; [apply LIB_STEP| ]. done. }
-    { lia. }
-    iMod (fupd_mask_mono with "EM_STEP") as (δ2 ℓ) "(EV & MSI & FUELS & ST & FR)"; [set_solver| ].
-    do 2 iExists _. iFrame "EV MSI".
+(*     rewrite -LASTE.  *)
+(*     iPoseProof (update_client_state with "[$] [$] [$] [$] [$]") as "EM_STEP"; eauto. *)
+(*     { eexists. split; [apply LIB_STEP| ]. done. } *)
+(*     { lia. } *)
+(*     iMod (fupd_mask_mono with "EM_STEP") as (δ2 ℓ) "(EV & MSI & FUELS & ST & FR)"; [set_solver| ]. *)
+(*     do 2 iExists _. iFrame "EV MSI". *)
 
-    iDestruct ("CLOS" with "[ST MSI_LIB YST_AUTH]") as "CLOS".
-    { iNext. iExists (_, _). rewrite /client_inv_impl. iFrame. }
-    iMod (fupd_mask_frame_r _ _ Einvs with "CLOS") as "_"; [set_solver| ].     
+(*     iDestruct ("CLOS" with "[ST MSI_LIB YST_AUTH]") as "CLOS". *)
+(*     { iNext. iExists (_, _). rewrite /client_inv_impl. iFrame. } *)
+(*     iMod (fupd_mask_frame_r _ _ Einvs with "CLOS") as "_"; [set_solver| ].      *)
 
-    iModIntro.
-    iDestruct "FUELS" as "[MAP FUEL]". iDestruct "FUELS_LIB" as "[MAP_LIB FUELS_LIB]".
-    rewrite /has_fuels. iSplitR "FUELS_LIB".
-    2: { rewrite dom_domain_restrict; [| set_solver]. done. }
-    simpl. rewrite dom_domain_restrict; [| set_solver].
-    rewrite /lib_pmi. do 3 iExists _. iFrame.
-    iSplitR; [done| ].
-    (* TODO: case when domain becomes empty *)
-    iLeft. iSplitR; [done| ].
-    rewrite TMAP_LIB. rewrite lookup_insert.
-    repeat erewrite @decide_False with (P := (Some (dom fs) = Some ∅)).
-    2-3: by intros [=].
-    iSplitR.
-    - iPureIntro. set_solver.
-    - rewrite dom_singleton_L big_sepS_singleton.
-      rewrite lookup_singleton. 
-      iDestruct "FUEL" as (?) "[%EQ ?]". inversion EQ. subst.  
-      iExists _. iFrame. iPureIntro. lia.
-  Qed.
+(*     iModIntro. *)
+(*     iDestruct "FUELS" as "[MAP FUEL]". iDestruct "FUELS_LIB" as "[MAP_LIB FUELS_LIB]". *)
+(*     rewrite /has_fuels. iSplitR "FUELS_LIB". *)
+(*     2: { rewrite dom_domain_restrict; [| set_solver]. done. } *)
+(*     simpl. rewrite dom_domain_restrict; [| set_solver]. *)
+(*     rewrite /lib_pmi. do 3 iExists _. iFrame. *)
+(*     iSplitR; [done| ]. *)
+(*     (* TODO: case when domain becomes empty *) *)
+(*     iLeft. iSplitR; [done| ]. *)
+(*     rewrite TMAP_LIB. rewrite lookup_insert. *)
+(*     repeat erewrite @decide_False with (P := (Some (dom fs) = Some ∅)). *)
+(*     2-3: by intros [=]. *)
+(*     iSplitR. *)
+(*     - iPureIntro. set_solver. *)
+(*     - rewrite dom_singleton_L big_sepS_singleton. *)
+(*       rewrite lookup_singleton.  *)
+(*       iDestruct "FUEL" as (?) "[%EQ ?]". inversion EQ. subst.   *)
+(*       iExists _. iFrame. iPureIntro. lia. *)
+(*   Qed. *)
   
-  Lemma model_step_lifting `{clientGS Σ} Einvs (DISJ_INV: Einvs ## ↑Ns):
-  LSG Einvs ∗ client_inv ⊢
-  ∀ (extr : execution_trace heap_lang) (auxtr : auxiliary_trace M)
-    (tp1 tp2 : list (language.expr heap_lang)) (σ1 σ2 : language.state heap_lang)
-    (s1 s2 : lib_model_impl) (fs1 fs2 : gmap (fmrole lib_model_impl) nat)
-    (ρ : fmrole lib_model_impl) (δ1 : M) (ζ : locale heap_lang)
-    (fr1 fr_stash : gset (fmrole lib_model_impl))
-    (_ : live_roles lib_model_impl s2 ∖ live_roles lib_model_impl s1 ⊆ fr1 ∪ dom fs1 ∩ dom fs2)
-    (_ : fr_stash ⊆ dom fs1) (_ : live_roles lib_model_impl s1
-                                  ∩ (fr_stash ∖ {[ρ]}) = ∅)
-    (_ : dom fs2 ∩ fr_stash = ∅) (_ : trace_last extr = (tp1, σ1))
-    (_ : trace_last auxtr = δ1) (_ : locale_step (tp1, σ1) (Some ζ) (tp2, σ2))
-    (_ : fmtrans lib_model_impl s1 (Some ρ) s2)
-    (_ : valid_new_fuelmap fs1 fs2 s1 s2 ρ (LM := lib_model))
-  ,
-    has_fuels ζ fs1 (PMPP := lib_PMPP) -∗
-    partial_model_is s1 (PartialModelPredicatesPre := lib_PMPP) -∗
-    em_msi (tp1, σ1) δ1 (em_GS0 := heap_fairnessGS) -∗
-    partial_free_roles_are fr1 (PartialModelPredicatesPre := lib_PMPP)
-    ={Einvs ∪ ↑Ns}=∗
-    ∃ (δ2 : M) (ℓ : mlabel M),
-      ⌜em_valid_state_evolution_fairness (extr :tr[ Some ζ ]: (tp2, σ2))
-         (auxtr :tr[ ℓ ]: δ2)⌝ ∗
-      has_fuels ζ fs2 (PMPP := lib_PMPP) ∗
-      partial_model_is s2 (PartialModelPredicatesPre := lib_PMPP) ∗
-      em_msi (tp2, σ2) δ2 (em_GS0 := heap_fairnessGS) ∗
-      partial_free_roles_are
-        (fr1 ∖ (live_roles lib_model_impl s2 ∖ (live_roles lib_model_impl s1 ∪ dom fs1 ∩ dom fs2))
-         ∪ fr_stash) (PartialModelPredicatesPre := lib_PMPP).
-  Proof.
-    iIntros "[#PMP #COMP]". iIntros "* FUELS_LIB ST_LIB MSI FR_LIB". simpl in *.
+(*   Lemma model_step_lifting `{clientGS Σ} Einvs (DISJ_INV: Einvs ## ↑Ns): *)
+(*   LSG Einvs ∗ client_inv ⊢ *)
+(*   ∀ (extr : execution_trace heap_lang) (auxtr : auxiliary_trace M) *)
+(*     (tp1 tp2 : list (language.expr heap_lang)) (σ1 σ2 : language.state heap_lang) *)
+(*     (s1 s2 : lib_model_impl) (fs1 fs2 : gmap (fmrole lib_model_impl) nat) *)
+(*     (ρ : fmrole lib_model_impl) (δ1 : M) (ζ : locale heap_lang) *)
+(*     (fr1 fr_stash : gset (fmrole lib_model_impl)) *)
+(*     (_ : live_roles lib_model_impl s2 ∖ live_roles lib_model_impl s1 ⊆ fr1 ∪ dom fs1 ∩ dom fs2) *)
+(*     (_ : fr_stash ⊆ dom fs1) (_ : live_roles lib_model_impl s1 *)
+(*                                   ∩ (fr_stash ∖ {[ρ]}) = ∅) *)
+(*     (_ : dom fs2 ∩ fr_stash = ∅) (_ : trace_last extr = (tp1, σ1)) *)
+(*     (_ : trace_last auxtr = δ1) (_ : locale_step (tp1, σ1) (Some ζ) (tp2, σ2)) *)
+(*     (_ : fmtrans lib_model_impl s1 (Some ρ) s2) *)
+(*     (_ : valid_new_fuelmap fs1 fs2 s1 s2 ρ (LM := lib_model)) *)
+(*   , *)
+(*     has_fuels ζ fs1 (PMPP := lib_PMPP) -∗ *)
+(*     partial_model_is s1 (PartialModelPredicatesPre := lib_PMPP) -∗ *)
+(*     em_msi (tp1, σ1) δ1 (em_GS0 := heap_fairnessGS) -∗ *)
+(*     partial_free_roles_are fr1 (PartialModelPredicatesPre := lib_PMPP) *)
+(*     ={Einvs ∪ ↑Ns}=∗ *)
+(*     ∃ (δ2 : M) (ℓ : mlabel M), *)
+(*       ⌜em_valid_state_evolution_fairness (extr :tr[ Some ζ ]: (tp2, σ2)) *)
+(*          (auxtr :tr[ ℓ ]: δ2)⌝ ∗ *)
+(*       has_fuels ζ fs2 (PMPP := lib_PMPP) ∗ *)
+(*       partial_model_is s2 (PartialModelPredicatesPre := lib_PMPP) ∗ *)
+(*       em_msi (tp2, σ2) δ2 (em_GS0 := heap_fairnessGS) ∗ *)
+(*       partial_free_roles_are *)
+(*         (fr1 ∖ (live_roles lib_model_impl s2 ∖ (live_roles lib_model_impl s1 ∪ dom fs1 ∩ dom fs2)) *)
+(*          ∪ fr_stash) (PartialModelPredicatesPre := lib_PMPP). *)
+(*   Proof. *)
+(*     iIntros "[#PMP #COMP]". iIntros "* FUELS_LIB ST_LIB MSI FR_LIB". simpl in *. *)
     
-    assert (ρ ∈ dom fs1) as DOM1ρ by apply x7.
-    assert (dom fs1 ≠ ∅ /\ fs1 ≠ ∅) as [FS1nz FS1nz'].
-    { split; intros ?; set_solver. }
+(*     assert (ρ ∈ dom fs1) as DOM1ρ by apply x7. *)
+(*     assert (dom fs1 ≠ ∅ /\ fs1 ≠ ∅) as [FS1nz FS1nz']. *)
+(*     { split; intros ?; set_solver. } *)
     
-    iPoseProof (lib_open_inv with "[$] FUELS_LIB") as "INV'"; [done| ]. 
-    rewrite union_comm_L. 
-    iMod (fupd_mask_frame_r _ _ Einvs with "INV'") as 
-      "(-> & (%lb & ST & inv') & LM & YST_AUTH & (%f & Ff & %BOUND) & MAP & FR & YST & FUEL_LIB & CLOS)"; [set_solver| ].
+(*     iPoseProof (lib_open_inv with "[$] FUELS_LIB") as "INV'"; [done| ].  *)
+(*     rewrite union_comm_L.  *)
+(*     iMod (fupd_mask_frame_r _ _ Einvs with "INV'") as  *)
+(*       "(-> & (%lb & ST & inv') & LM & YST_AUTH & (%f & Ff & %BOUND) & MAP & FR & YST & FUEL_LIB & CLOS)"; [set_solver| ]. *)
     
-    iMod (actual_update_step_still_alive with "[LM FUEL_LIB] [$] [$] [$]") as "LIFT"; eauto.
-    { rewrite has_fuels_equiv. iFrame. iApply frag_fuel_is_big_sepM; done. }
-    iDestruct "LIFT" as (lb') "(%LIB_STEP & FUELS_LIB & ST_LIB & MSI_LIB & FR_LIB & %TMAP_LIB)".
-    simpl. iFrame "ST_LIB".
+(*     iMod (actual_update_step_still_alive with "[LM FUEL_LIB] [$] [$] [$]") as "LIFT"; eauto. *)
+(*     { rewrite has_fuels_equiv. iFrame. iApply frag_fuel_is_big_sepM; done. } *)
+(*     iDestruct "LIFT" as (lb') "(%LIB_STEP & FUELS_LIB & ST_LIB & MSI_LIB & FR_LIB & %TMAP_LIB)". *)
+(*     simpl. iFrame "ST_LIB". *)
     
-    iAssert (has_fuels 0 {[ inl ρlg := f ]}) with "[MAP Ff]" as "FUELS".
-    { rewrite /has_fuels. rewrite dom_singleton_L big_sepS_singleton.
-      rewrite lookup_singleton. iFrame. iExists _. iFrame. done. }
+(*     iAssert (has_fuels 0 {[ inl ρlg := f ]}) with "[MAP Ff]" as "FUELS". *)
+(*     { rewrite /has_fuels. rewrite dom_singleton_L big_sepS_singleton. *)
+(*       rewrite lookup_singleton. iFrame. iExists _. iFrame. done. } *)
 
-    rewrite -x3 -x4. rewrite -x3 in x5. 
-    iPoseProof (update_client_state with "[$] [MSI] [ST] [$] [$]") as "EM_STEP"; eauto.
-    { eexists. split; [apply LIB_STEP| ]. done. }
-    { lia. }
-    iMod (fupd_mask_mono with "EM_STEP") as (δ2 ℓ) "(EV & MSI & FUELS & ST & FR)"; [set_solver| ].
-    do 2 iExists _. iFrame "EV MSI".
+(*     rewrite -x3 -x4. rewrite -x3 in x5.  *)
+(*     iPoseProof (update_client_state with "[$] [MSI] [ST] [$] [$]") as "EM_STEP"; eauto. *)
+(*     { eexists. split; [apply LIB_STEP| ]. done. } *)
+(*     { lia. } *)
+(*     iMod (fupd_mask_mono with "EM_STEP") as (δ2 ℓ) "(EV & MSI & FUELS & ST & FR)"; [set_solver| ]. *)
+(*     do 2 iExists _. iFrame "EV MSI". *)
 
-    iDestruct ("CLOS" with "[ST MSI_LIB YST_AUTH]") as "CLOS".
-    { iNext. iExists (_, _). rewrite /client_inv_impl. iFrame. }
-    iMod (fupd_mask_frame_r _ _ Einvs with "CLOS") as "_"; [set_solver| ].
-    iModIntro.
+(*     iDestruct ("CLOS" with "[ST MSI_LIB YST_AUTH]") as "CLOS". *)
+(*     { iNext. iExists (_, _). rewrite /client_inv_impl. iFrame. } *)
+(*     iMod (fupd_mask_frame_r _ _ Einvs with "CLOS") as "_"; [set_solver| ]. *)
+(*     iModIntro. *)
 
-    rewrite !has_fuels_equiv. simpl.
-    iDestruct "FUELS" as "[MAP FUELS]".
-    iDestruct "FUELS_LIB" as "[MAP' FUELS_LIB]". iFrame "FUELS_LIB FR_LIB".
-    rewrite /lib_pmi. do 3 iExists _. iFrame.
-    iSplitR; [done |].
-    rewrite TMAP_LIB. rewrite lookup_insert.
-    dEq.
-    - iRight. rewrite big_sepM_singleton. iFrame.
-      iPureIntro. set_solver. 
-    - iLeft. rewrite big_sepM_singleton.
-      iApply bi.sep_assoc. iSplitR "FUELS".
-      2: { iExists _. iFrame. iPureIntro. lia. }
-      iPureIntro. split; [| set_solver]. intros ?. rewrite H1 in n. done.
-  Qed.
-
-
-  Lemma lib_PMP `{clientGS Σ} Einvs (DISJ_INV: Einvs ## ↑Ns):
-    LSG Einvs ∗ client_inv ⊢
-    (* PartialModelPredicates (Einvs ∪ ↑Ns) (LM := LM) (iLM := spinlock_model) (PMPP := (sl1_PMPP γ)).  *)
-    PartialModelPredicates (Einvs ∪ ↑Ns) (EM := EM) (iLM := lib_model) (PMPP := lib_PMPP) (eGS := heap_fairnessGS).
-  Proof. 
-    iIntros "[#PMP #COMP]". iApply @Build_PartialModelPredicates.
-
-    iModIntro. repeat iSplitR.
-    - iIntros "* FUELS_LIB MSI".
-      iDestruct (fuel_step_lifting with "[$] [] [] FUELS_LIB MSI") as "LIFT"; eauto.
-      (* change the PMP interface so it allows fupd in fuel step *)
-      admit.
-    - (* TODO: shouldn't be required from a library that doesn't fork *)
-      admit.
-    - iIntros "* FUELS_LIB ST MSI FR". 
-      iApply (model_step_lifting with "[$] [] [] [] [] [] [] [] [] [] [$] [$] [$] [$]"); eauto.
-  Admitted.
-
-  (* TODO: problems with Countable instance *)
-  (* Set Printing All. *)
-  (* Lemma fuel_reorder_preserves_client_LSI: *)
-  (*   fuel_reorder_preserves_LSI (LSI := client_LSI).  *)
-  Lemma fuel_reorder_preserves_client_LSI:
-    @fuel_reorder_preserves_LSI (locale heap_lang) client_model_impl client_LSI.
-  Proof. 
-    red. rewrite /client_LSI. intros. set_solver.
-  Qed. 
+(*     rewrite !has_fuels_equiv. simpl. *)
+(*     iDestruct "FUELS" as "[MAP FUELS]". *)
+(*     iDestruct "FUELS_LIB" as "[MAP' FUELS_LIB]". iFrame "FUELS_LIB FR_LIB". *)
+(*     rewrite /lib_pmi. do 3 iExists _. iFrame. *)
+(*     iSplitR; [done |]. *)
+(*     rewrite TMAP_LIB. rewrite lookup_insert. *)
+(*     dEq. *)
+(*     - iRight. rewrite big_sepM_singleton. iFrame. *)
+(*       iPureIntro. set_solver.  *)
+(*     - iLeft. rewrite big_sepM_singleton. *)
+(*       iApply bi.sep_assoc. iSplitR "FUELS". *)
+(*       2: { iExists _. iFrame. iPureIntro. lia. } *)
+(*       iPureIntro. split; [| set_solver]. intros ?. rewrite H1 in n. done. *)
+(*   Qed. *)
 
 
-  Notation "'sub' d" := (fun n => n - d) (at level 10). 
+(*   Lemma lib_PMP `{clientGS Σ} Einvs (DISJ_INV: Einvs ## ↑Ns): *)
+(*     LSG Einvs ∗ client_inv ⊢ *)
+(*     (* PartialModelPredicates (Einvs ∪ ↑Ns) (LM := LM) (iLM := spinlock_model) (PMPP := (sl1_PMPP γ)).  *) *)
+(*     PartialModelPredicates (Einvs ∪ ↑Ns) (EM := EM) (iLM := lib_model) (PMPP := lib_PMPP) (eGS := heap_fairnessGS). *)
+(*   Proof.  *)
+(*     iIntros "[#PMP #COMP]". iApply @Build_PartialModelPredicates. *)
 
-  Lemma sub_comp `{Countable K} (fs: gmap K nat) (d1 d2: nat):
-    (sub d1 ∘ sub d2) <$> fs = sub (d1 + d2) <$> fs.
-  Proof.
-    apply leibniz_equiv. apply map_fmap_proper; [| done].
-    intros ??->. apply leibniz_equiv_iff.
-    rewrite /compose. lia. 
-  Qed.
+(*     iModIntro. repeat iSplitR. *)
+(*     - iIntros "* FUELS_LIB MSI". *)
+(*       iDestruct (fuel_step_lifting with "[$] [] [] FUELS_LIB MSI") as "LIFT"; eauto. *)
+(*       (* change the PMP interface so it allows fupd in fuel step *) *)
+(*       admit. *)
+(*     - (* TODO: shouldn't be required from a library that doesn't fork *) *)
+(*       admit. *)
+(*     - iIntros "* FUELS_LIB ST MSI FR".  *)
+(*       iApply (model_step_lifting with "[$] [] [] [] [] [] [] [] [] [] [$] [$] [$] [$]"); eauto. *)
+(*   Admitted. *)
 
-  Lemma sub_0_id `{Countable K} (fs: gmap K nat):
-    fs = sub 0 <$> fs.
-  Proof.
-    rewrite -{1}(map_fmap_id fs).
-    apply leibniz_equiv. apply map_fmap_proper; [| done].
-    intros ??->. apply leibniz_equiv_iff.
-    simpl. lia.
-  Qed.
+(*   (* TODO: problems with Countable instance *) *)
+(*   (* Set Printing All. *) *)
+(*   (* Lemma fuel_reorder_preserves_client_LSI: *) *)
+(*   (*   fuel_reorder_preserves_LSI (LSI := client_LSI).  *) *)
+(*   Lemma fuel_reorder_preserves_client_LSI: *)
+(*     @fuel_reorder_preserves_LSI (locale heap_lang) client_model_impl client_LSI. *)
+(*   Proof.  *)
+(*     red. rewrite /client_LSI. intros. set_solver. *)
+(*   Qed.  *)
 
-  Ltac solve_fuels_ge_1 FS := 
-    intros ?? [? [<- GE]]%lookup_fmap_Some; apply FS in GE; simpl; lia.
+
+(*   Notation "'sub' d" := (fun n => n - d) (at level 10).  *)
+
+(*   Lemma sub_comp `{Countable K} (fs: gmap K nat) (d1 d2: nat): *)
+(*     (sub d1 ∘ sub d2) <$> fs = sub (d1 + d2) <$> fs. *)
+(*   Proof. *)
+(*     apply leibniz_equiv. apply map_fmap_proper; [| done]. *)
+(*     intros ??->. apply leibniz_equiv_iff. *)
+(*     rewrite /compose. lia.  *)
+(*   Qed. *)
+
+(*   Lemma sub_0_id `{Countable K} (fs: gmap K nat): *)
+(*     fs = sub 0 <$> fs. *)
+(*   Proof. *)
+(*     rewrite -{1}(map_fmap_id fs). *)
+(*     apply leibniz_equiv. apply map_fmap_proper; [| done]. *)
+(*     intros ??->. apply leibniz_equiv_iff. *)
+(*     simpl. lia. *)
+(*   Qed. *)
+
+(*   Ltac solve_fuels_ge_1 FS :=  *)
+(*     intros ?? [? [<- GE]]%lookup_fmap_Some; apply FS in GE; simpl; lia. *)
   
-  Ltac solve_fuels_S FS :=    
-    iDestruct (has_fuels_gt_1 with "FUELS") as "F";
-    [| rewrite -map_fmap_compose; (try rewrite sub_comp); by iFrame];
-    solve_fuels_ge_1 FS. 
+(*   Ltac solve_fuels_S FS :=     *)
+(*     iDestruct (has_fuels_gt_1 with "FUELS") as "F"; *)
+(*     [| rewrite -map_fmap_compose; (try rewrite sub_comp); by iFrame]; *)
+(*     solve_fuels_ge_1 FS.  *)
 
-  Ltac solve_map_not_empty := intros ?MM%fmap_empty_iff; try rewrite -insert_empty in MM; try apply insert_non_empty in MM; set_solver. 
+(*   Ltac solve_map_not_empty := intros ?MM%fmap_empty_iff; try rewrite -insert_empty in MM; try apply insert_non_empty in MM; set_solver.  *)
 
-  Ltac pure_step_impl FS :=
-    try rewrite sub_comp;
-    iApply wp_lift_pure_step_no_fork; auto;
-    [| iSplitR; [done| ]; do 3 iModIntro; iSplitL "FUELS"];
-    [| solve_fuels_S FS |];
-    (* [by intros ?%fmap_empty_iff| ]; *)
-    [solve_map_not_empty| ];
-    iIntros "FUELS"; simpl; try rewrite sub_comp. 
+(*   Ltac pure_step_impl FS := *)
+(*     try rewrite sub_comp; *)
+(*     iApply wp_lift_pure_step_no_fork; auto; *)
+(*     [| iSplitR; [done| ]; do 3 iModIntro; iSplitL "FUELS"]; *)
+(*     [| solve_fuels_S FS |]; *)
+(*     (* [by intros ?%fmap_empty_iff| ]; *) *)
+(*     [solve_map_not_empty| ]; *)
+(*     iIntros "FUELS"; simpl; try rewrite sub_comp.  *)
 
-  Ltac pure_step FS :=
-    unshelve (pure_step_impl FS); [by apply fuel_reorder_preserves_client_LSI| ].
+(*   Ltac pure_step FS := *)
+(*     unshelve (pure_step_impl FS); [by apply fuel_reorder_preserves_client_LSI| ]. *)
 
-  (* TODO: move, upstream *)
-  Lemma dom_filter_comm {K A: Type} `{Countable K}
-                        (P: K -> Prop) `{∀ x : K, Decision (P x)}:
-    forall (m: gmap K A), dom (filter (fun '(k, _) => P k) m) = filter P (dom m).
-  Proof. 
-    intros. apply leibniz_equiv. apply dom_filter. intros.
-    rewrite elem_of_filter elem_of_dom.
-    rewrite /is_Some. split; [intros [?[??]] | intros [? [??]]]; eauto.
-  Qed. 
+(*   (* TODO: move, upstream *) *)
+(*   Lemma dom_filter_comm {K A: Type} `{Countable K} *)
+(*                         (P: K -> Prop) `{∀ x : K, Decision (P x)}: *)
+(*     forall (m: gmap K A), dom (filter (fun '(k, _) => P k) m) = filter P (dom m). *)
+(*   Proof.  *)
+(*     intros. apply leibniz_equiv. apply dom_filter. intros. *)
+(*     rewrite elem_of_filter elem_of_dom. *)
+(*     rewrite /is_Some. split; [intros [?[??]] | intros [? [??]]]; eauto. *)
+(*   Qed.  *)
 
-Lemma client_spec (Einvs: coPset) (lb0: fmstate lib_fair) f
-    (FB: f >= client_fl)
-    (* TODO: get rid of these restrictions *)
-    (DISJ_INV1: Einvs ## ↑Ns)
-    (* (DISJ_INV2: Einvs ## ↑nroot.@"spinlock"): *)    
-    (LB0_INFO: lib_ls_premise lb0)
-    :
-    LSG Einvs -∗
-    {{{ partial_model_is (lb0, 2)  ∗ 
-        partial_free_roles_are {[ inl ρlg ]} ∗ 
-        has_fuels 0 {[ inr ρy := f ]} (PMPP := PMPP)  }}}
-      client #() @ 0
-    {{{ RET #(); partial_mapping_is {[ 0 := ∅ ]} }}}.
-  Proof using cpG.
-    unfold client_fl in *. 
-    iIntros "#PMP" (Φ) "!> (ST & FREE & FUELS) POST". rewrite /client.
+(* Lemma client_spec (Einvs: coPset) (lb0: fmstate lib_fair) f *)
+(*     (FB: f >= client_fl) *)
+(*     (* TODO: get rid of these restrictions *) *)
+(*     (DISJ_INV1: Einvs ## ↑Ns) *)
+(*     (* (DISJ_INV2: Einvs ## ↑nroot.@"spinlock"): *)     *)
+(*     (LB0_INFO: lib_ls_premise lb0) *)
+(*     : *)
+(*     LSG Einvs -∗ *)
+(*     {{{ partial_model_is (lb0, 2)  ∗  *)
+(*         partial_free_roles_are {[ inl ρlg ]} ∗  *)
+(*         has_fuels 0 {[ inr ρy := f ]} (PMPP := PMPP)  }}} *)
+(*       client #() @ 0 *)
+(*     {{{ RET #(); partial_mapping_is {[ 0 := ∅ ]} }}}. *)
+(*   Proof using cpG. *)
+(*     unfold client_fl in *.  *)
+(*     iIntros "#PMP" (Φ) "!> (ST & FREE & FUELS) POST". rewrite /client. *)
 
-    rewrite (sub_0_id {[ _ := _ ]}). 
-    assert (fuels_ge ({[inr ρy := f]}: gmap (fmrole client_model_impl) nat) 10) as FS.
-    { red. intros ??[<- ->]%lookup_singleton_Some. lia. }
+(*     rewrite (sub_0_id {[ _ := _ ]}).  *)
+(*     assert (fuels_ge ({[inr ρy := f]}: gmap (fmrole client_model_impl) nat) 10) as FS. *)
+(*     { red. intros ??[<- ->]%lookup_singleton_Some. lia. } *)
 
-    pure_step FS.
+(*     pure_step FS. *)
 
-    wp_bind (ref _)%E.
-    iApply (wp_alloc_nostep with "[$] [FUELS]").
-    2: { solve_fuels_S FS. }
-    { solve_map_not_empty. }
-    iNext. iIntros (l) "(L & MT & FUELS) /=".
-    Unshelve. 2: by apply fuel_reorder_preserves_client_LSI.
+(*     wp_bind (ref _)%E. *)
+(*     iApply (wp_alloc_nostep with "[$] [FUELS]"). *)
+(*     2: { solve_fuels_S FS. } *)
+(*     { solve_map_not_empty. } *)
+(*     iNext. iIntros (l) "(L & MT & FUELS) /=". *)
+(*     Unshelve. 2: by apply fuel_reorder_preserves_client_LSI. *)
 
-    pure_step FS. pure_step FS.
-    (* Set Printing Implicit. Unshelve. *)
+(*     pure_step FS. pure_step FS. *)
+(*     (* Set Printing Implicit. Unshelve. *) *)
 
-    pose proof (live_roles_2 lb0) as LIVE2.
-    pose proof (live_roles_1 lb0) as LIVE1.
-    (* TODO: after introduction of external transitions,
-       here the false branch should be used *)
-    pose proof (lib_premise_dis _ LB0_INFO) as LIB_LIVE. 
-    rewrite decide_True in LIVE1; [ | done]. 
+(*     pose proof (live_roles_2 lb0) as LIVE2. *)
+(*     pose proof (live_roles_1 lb0) as LIVE1. *)
+(*     (* TODO: after introduction of external transitions, *)
+(*        here the false branch should be used *) *)
+(*     pose proof (lib_premise_dis _ LB0_INFO) as LIB_LIVE.  *)
+(*     rewrite decide_True in LIVE1; [ | done].  *)
 
-    wp_bind (_ <- _)%E.
-    iApply (wp_store_step_keep with "[$] [L ST FUELS FREE]").
-    { set_solver. }
-    8: { iFrame "L ST FREE". iNext.
-         rewrite map_fmap_singleton. iFrame. }
-    { econstructor. }
-    3: { rewrite dom_singleton. reflexivity. }
-    2: { rewrite LIVE2 LIVE1.
-         apply union_subseteq_l'. set_solver. } 
-    2: { set_solver. }
-    { Unshelve. 2: exact {[ inl ρlg := lm_fl client_model (lb0, 1) ]}.
-      repeat split; rewrite ?LIVE2 ?LIVE1.
-      1-3, 5-7: set_solver. 
-      intros. assert (ρ' = inl ρlg) as -> by set_solver.
-      rewrite lookup_singleton. simpl. lia. }
-    { set_solver. }
-    { red. intros. simpl. red.
-      intros.
-      (* assert (client_LSI (lb0, 2) M0 F) as LSI1 by admit. *)
-      (* red in LSI1. *)
-      rewrite /update_mapping. rewrite map_imap_dom_eq.
-      2: { intros. destruct decide; [| done].
-           by apply elem_of_dom. }
-      rewrite dom_gset_to_gmap.
-      rewrite !dom_singleton.
-      assert (gi = ρlg) as ->.
-      { by destruct gi, ρlg. }
-      set_solver. }
+(*     wp_bind (_ <- _)%E. *)
+(*     iApply (wp_store_step_keep with "[$] [L ST FUELS FREE]"). *)
+(*     { set_solver. } *)
+(*     8: { iFrame "L ST FREE". iNext. *)
+(*          rewrite map_fmap_singleton. iFrame. } *)
+(*     { econstructor. } *)
+(*     3: { rewrite dom_singleton. reflexivity. } *)
+(*     2: { rewrite LIVE2 LIVE1. *)
+(*          apply union_subseteq_l'. set_solver. }  *)
+(*     2: { set_solver. } *)
+(*     { Unshelve. 2: exact {[ inl ρlg := lm_fl client_model (lb0, 1) ]}. *)
+(*       repeat split; rewrite ?LIVE2 ?LIVE1. *)
+(*       1-3, 5-7: set_solver.  *)
+(*       intros. assert (ρ' = inl ρlg) as -> by set_solver. *)
+(*       rewrite lookup_singleton. simpl. lia. } *)
+(*     { set_solver. } *)
+(*     { red. intros. simpl. red. *)
+(*       intros. *)
+(*       (* assert (client_LSI (lb0, 2) M0 F) as LSI1 by admit. *) *)
+(*       (* red in LSI1. *) *)
+(*       rewrite /update_mapping. rewrite map_imap_dom_eq. *)
+(*       2: { intros. destruct decide; [| done]. *)
+(*            by apply elem_of_dom. } *)
+(*       rewrite dom_gset_to_gmap. *)
+(*       rewrite !dom_singleton. *)
+(*       assert (gi = ρlg) as ->. *)
+(*       { by destruct gi, ρlg. } *)
+(*       set_solver. } *)
 
-    iNext. iIntros "(L & ST & FUELS & FR)".
-    rewrite LIVE2 LIVE1.
-    iDestruct (partial_free_roles_are_Proper with "FR") as "FR".
-    { rewrite subseteq_empty_difference; [| set_solver].
-      rewrite union_empty_l. reflexivity. }
+(*     iNext. iIntros "(L & ST & FUELS & FR)". *)
+(*     rewrite LIVE2 LIVE1. *)
+(*     iDestruct (partial_free_roles_are_Proper with "FR") as "FR". *)
+(*     { rewrite subseteq_empty_difference; [| set_solver]. *)
+(*       rewrite union_empty_l. reflexivity. } *)
 
-    simpl. clear FS. 
-    rewrite (sub_0_id {[ _ := _ ]}).
-    assert (fuels_ge ({[inl ρlg := client_fl]}: gmap (fmrole client_model_impl) nat) 10) as FS.
-    { red. unfold client_fl. 
-      intros ??[? ?]%lookup_singleton_Some. lia. }
+(*     simpl. clear FS.  *)
+(*     rewrite (sub_0_id {[ _ := _ ]}). *)
+(*     assert (fuels_ge ({[inl ρlg := client_fl]}: gmap (fmrole client_model_impl) nat) 10) as FS. *)
+(*     { red. unfold client_fl.  *)
+(*       intros ??[? ?]%lookup_singleton_Some. lia. } *)
 
-    do 2 pure_step FS. 
+(*     do 2 pure_step FS.  *)
 
-    iApply fupd_wp.
-    iPoseProof (init_client_inv with "ST") as "inv". 
-    iMod (fupd_mask_mono with "inv") as (?) "(#INV & LF & LM & LST & LFR & YST)".
-    { set_solver. }
-    iModIntro. 
+(*     iApply fupd_wp. *)
+(*     iPoseProof (init_client_inv with "ST") as "inv".  *)
+(*     iMod (fupd_mask_mono with "inv") as (?) "(#INV & LF & LM & LST & LFR & YST)". *)
+(*     { set_solver. } *)
+(*     iModIntro.  *)
 
-    wp_bind (lib_fun #())%E.
-    (* iDestruct "FUELS" as "[MAP FUELS]".  *)
-    iDestruct (has_fuels_equiv with "FUELS") as "[MAP FUELS]".
-    iApply (lib_spec with "[] [LST YST LF LM FR MAP FUELS]").
-    { iApply lib_PMP; [done| ]. iSplit; done. }
-    { simpl.
-      iDestruct (lib_premise with "LST LF LM") as "(LST & LF & LM)"; eauto.       
-      rewrite has_fuels_equiv. simpl. 
-      rewrite dom_singleton_L !big_sepM_singleton.
-      iFrame.
-      do 3 iExists _. iFrame. iSplitR.
-      { eauto. }
-      iLeft.
-      rewrite bi.sep_assoc. iSplitR.
-      { iPureIntro. set_solver. }
-      rewrite !map_fmap_singleton big_sepM_singleton.
-      iExists _. iFrame. iPureIntro. rewrite /client_fl. lia. }
+(*     wp_bind (lib_fun #())%E. *)
+(*     (* iDestruct "FUELS" as "[MAP FUELS]".  *) *)
+(*     iDestruct (has_fuels_equiv with "FUELS") as "[MAP FUELS]". *)
+(*     iApply (lib_spec with "[] [LST YST LF LM FR MAP FUELS]"). *)
+(*     { iApply lib_PMP; [done| ]. iSplit; done. } *)
+(*     { simpl. *)
+(*       iDestruct (lib_premise with "LST LF LM") as "(LST & LF & LM)"; eauto.        *)
+(*       rewrite has_fuels_equiv. simpl.  *)
+(*       rewrite dom_singleton_L !big_sepM_singleton. *)
+(*       iFrame. *)
+(*       do 3 iExists _. iFrame. iSplitR. *)
+(*       { eauto. } *)
+(*       iLeft. *)
+(*       rewrite bi.sep_assoc. iSplitR. *)
+(*       { iPureIntro. set_solver. } *)
+(*       rewrite !map_fmap_singleton big_sepM_singleton. *)
+(*       iExists _. iFrame. iPureIntro. rewrite /client_fl. lia. } *)
  
-    iNext. iIntros "[LMAP LFR']". simpl. 
-    iDestruct "LMAP" as (???) "(%LIBM&LM&MATCH&MAP&FR&YST)".
-    assert (L = ∅) as -> by set_solver.
-    iDestruct "MATCH" as "[[%?] | (_&[->->]&FUEL')]"; [set_solver| ]. clear LIBM.
+(*     iNext. iIntros "[LMAP LFR']". simpl.  *)
+(*     iDestruct "LMAP" as (???) "(%LIBM&LM&MATCH&MAP&FR&YST)". *)
+(*     assert (L = ∅) as -> by set_solver. *)
+(*     iDestruct "MATCH" as "[[%?] | (_&[->->]&FUEL')]"; [set_solver| ]. clear LIBM. *)
                                       
-    iAssert (has_fuels 0 {[ inr ρy := 15 ]})%I with "[FUEL' MAP]" as "FUELS".
-    { rewrite /has_fuels.
-      rewrite !dom_singleton_L !big_sepS_singleton.
-      rewrite lookup_singleton. iFrame. iExists _. iFrame. done. }
+(*     iAssert (has_fuels 0 {[ inr ρy := 15 ]})%I with "[FUEL' MAP]" as "FUELS". *)
+(*     { rewrite /has_fuels. *)
+(*       rewrite !dom_singleton_L !big_sepS_singleton. *)
+(*       rewrite lookup_singleton. iFrame. iExists _. iFrame. done. } *)
     
-    simpl. clear FS. 
-    rewrite (sub_0_id {[ inr ρy := _ ]}).
-    assert (fuels_ge ({[ inr ρy := 15 ]}: gmap (fmrole client_model_impl) nat) 10) as FS.
-    { red. intros ??[? ?]%lookup_singleton_Some. lia. }
+(*     simpl. clear FS.  *)
+(*     rewrite (sub_0_id {[ inr ρy := _ ]}). *)
+(*     assert (fuels_ge ({[ inr ρy := 15 ]}: gmap (fmrole client_model_impl) nat) 10) as FS. *)
+(*     { red. intros ??[? ?]%lookup_singleton_Some. lia. } *)
 
-    pure_step FS. pure_step FS.
+(*     pure_step FS. pure_step FS. *)
     
-    wp_bind (_ <- _)%E.
+(*     wp_bind (_ <- _)%E. *)
 
-    iApply wp_atomic.
-    iInv Ns as ((lb, y)) "inv" "CLOS". rewrite {1}/client_inv_impl. 
-    iDestruct "inv" as "(>ST & >YST_AUTH & > inv')".
-    iAssert (⌜ y = 1 ⌝)%I as %->.
-    { iCombine "YST_AUTH YST" as "Y". iDestruct (own_valid with "Y") as %V.
-      apply auth_both_valid_discrete in V as [EQ%Excl_included _]. done. }
-    iAssert (⌜ ls_tmap lb !! ρlg = Some ∅ ⌝)%I as %LIB_END.
-    { iApply (frag_mapping_same with "[inv'] LM"). 
-      rewrite /model_state_interp. iFrame.
-      iDestruct "inv'" as (?) "(?&?&_)". iFrame.  }
+(*     iApply wp_atomic. *)
+(*     iInv Ns as ((lb, y)) "inv" "CLOS". rewrite {1}/client_inv_impl.  *)
+(*     iDestruct "inv" as "(>ST & >YST_AUTH & > inv')". *)
+(*     iAssert (⌜ y = 1 ⌝)%I as %->. *)
+(*     { iCombine "YST_AUTH YST" as "Y". iDestruct (own_valid with "Y") as %V. *)
+(*       apply auth_both_valid_discrete in V as [EQ%Excl_included _]. done. } *)
+(*     iAssert (⌜ ls_tmap lb !! ρlg = Some ∅ ⌝)%I as %LIB_END. *)
+(*     { iApply (frag_mapping_same with "[inv'] LM").  *)
+(*       rewrite /model_state_interp. iFrame. *)
+(*       iDestruct "inv'" as (?) "(?&?&_)". iFrame.  } *)
 
-    pose proof (live_roles_1 lb) as LIVE1'. 
-    (* rewrite !(decide_False, decide_True) in LIVE1'. -- TODO: how to do it in ssr?*)
-    erewrite decide_False, decide_True in LIVE1'; eauto.
-    2: { apply LM_map_empty_notlive. eauto. }    
+(*     pose proof (live_roles_1 lb) as LIVE1'.  *)
+(*     (* rewrite !(decide_False, decide_True) in LIVE1'. -- TODO: how to do it in ssr?*) *)
+(*     erewrite decide_False, decide_True in LIVE1'; eauto. *)
+(*     2: { apply LM_map_empty_notlive. eauto. }     *)
     
-    pose proof (live_roles_0 lb) as LIVE0. 
+(*     pose proof (live_roles_0 lb) as LIVE0.  *)
     
-    iModIntro. 
-    iApply (wp_store_step_singlerole_keep with "[$] [L ST FUELS]").
-    { set_solver. }
-    (* { reflexivity. } *)
-    6: { iFrame "L ST". iNext.
-         iApply has_fuel_fuels. rewrite map_fmap_singleton. iFrame. }
-    2: { by apply ct_y_step_1. }
-    3: { rewrite LIVE1' LIVE0. set_solver. }
-    { Unshelve. 2: exact 7. simpl. rewrite /client_fl. lia. }
-    { lia. }
-    { red. intros. simpl. red.
-      intros ? [? MAP].
-      apply (ls_mapping_tmap_corr (LM := lib_model)) in MAP as (? & TMAP' & ?).
-      assert (ρlg = gi) as <- by (by destruct ρlg, gi).
-      set_solver. }
+(*     iModIntro.  *)
+(*     iApply (wp_store_step_singlerole_keep with "[$] [L ST FUELS]"). *)
+(*     { set_solver. } *)
+(*     (* { reflexivity. } *) *)
+(*     6: { iFrame "L ST". iNext. *)
+(*          iApply has_fuel_fuels. rewrite map_fmap_singleton. iFrame. } *)
+(*     2: { by apply ct_y_step_1. } *)
+(*     3: { rewrite LIVE1' LIVE0. set_solver. } *)
+(*     { Unshelve. 2: exact 7. simpl. rewrite /client_fl. lia. } *)
+(*     { lia. } *)
+(*     { red. intros. simpl. red. *)
+(*       intros ? [? MAP]. *)
+(*       apply (ls_mapping_tmap_corr (LM := lib_model)) in MAP as (? & TMAP' & ?). *)
+(*       assert (ρlg = gi) as <- by (by destruct ρlg, gi). *)
+(*       set_solver. } *)
 
-    (* rewrite LIVE0. erewrite decide_False; [| set_solver]. *)
-    iNext. iIntros "(L & ST & FUELS)".    
-    iMod (y_update_model _ _ 0 with "YST_AUTH YST") as "[YST_AUTH YST]".
+(*     (* rewrite LIVE0. erewrite decide_False; [| set_solver]. *) *)
+(*     iNext. iIntros "(L & ST & FUELS)".     *)
+(*     iMod (y_update_model _ _ 0 with "YST_AUTH YST") as "[YST_AUTH YST]". *)
     
-    iMod ("CLOS" with "[YST_AUTH ST inv']") as "_".
-    { iNext. iExists (_, _). rewrite /client_inv_impl. iFrame. }
-    iModIntro.
+(*     iMod ("CLOS" with "[YST_AUTH ST inv']") as "_". *)
+(*     { iNext. iExists (_, _). rewrite /client_inv_impl. iFrame. } *)
+(*     iModIntro. *)
 
-    iDestruct (has_fuel_fuels with "FUELS") as "FUELS". 
-    simpl. clear FS. 
-    rewrite (sub_0_id {[ inr ρy := _ ]}).
-    assert (fuels_ge ({[ inr ρy := 7 ]}: gmap (fmrole client_model_impl) nat) 7) as FS.
-    { red. intros ??[<- ->]%lookup_singleton_Some. lia. }
+(*     iDestruct (has_fuel_fuels with "FUELS") as "FUELS".  *)
+(*     simpl. clear FS.  *)
+(*     rewrite (sub_0_id {[ inr ρy := _ ]}). *)
+(*     assert (fuels_ge ({[ inr ρy := 7 ]}: gmap (fmrole client_model_impl) nat) 7) as FS. *)
+(*     { red. intros ??[<- ->]%lookup_singleton_Some. lia. } *)
 
-    do 2 pure_step FS.
+(*     do 2 pure_step FS. *)
 
-    iApply wp_atomic. 
-    iInv Ns as ((lb', y)) "inv" "CLOS". rewrite {1}/client_inv_impl. 
-    iDestruct "inv" as "(>ST & >YST_AUTH & > inv')".
-    iAssert (⌜ y = 0 ⌝)%I as %->.
-    { iCombine "YST_AUTH YST" as "Y". iDestruct (own_valid with "Y") as %V.
-      apply auth_both_valid_discrete in V as [EQ%Excl_included _]. done. }
+(*     iApply wp_atomic.  *)
+(*     iInv Ns as ((lb', y)) "inv" "CLOS". rewrite {1}/client_inv_impl.  *)
+(*     iDestruct "inv" as "(>ST & >YST_AUTH & > inv')". *)
+(*     iAssert (⌜ y = 0 ⌝)%I as %->. *)
+(*     { iCombine "YST_AUTH YST" as "Y". iDestruct (own_valid with "Y") as %V. *)
+(*       apply auth_both_valid_discrete in V as [EQ%Excl_included _]. done. } *)
 
-    (* Unshelve. 2: exact (⊤ ∖ ↑Ns).  *)
-    iModIntro.
+(*     (* Unshelve. 2: exact (⊤ ∖ ↑Ns).  *) *)
+(*     iModIntro. *)
     
-    iApply (wp_lift_pure_step_no_fork_remove_role {[ inr ρy ]} ((lb', 0): fmstate client_model_impl) _ _ _ _ _ _ _ (sub 3 <$> {[inr ρy := 7]}) (iLM := client_model)); eauto.
-    { solve_map_not_empty. }
-    { set_solver. }
-    { rewrite live_roles_0. set_solver. }
-    { red. intros. red. intros.
-      red in H0. specialize (H0 _ H1). 
-      rewrite dom_filter_comm. apply elem_of_filter. split; set_solver. }
-    iFrame "PMP". do 3 iModIntro. iFrame.
-    iSplitL "FUELS".
-    { solve_fuels_S FS. } 
-    iIntros "ST FUELS". 
+(*     iApply (wp_lift_pure_step_no_fork_remove_role {[ inr ρy ]} ((lb', 0): fmstate client_model_impl) _ _ _ _ _ _ _ (sub 3 <$> {[inr ρy := 7]}) (iLM := client_model)); eauto. *)
+(*     { solve_map_not_empty. } *)
+(*     { set_solver. } *)
+(*     { rewrite live_roles_0. set_solver. } *)
+(*     { red. intros. red. intros. *)
+(*       red in H0. specialize (H0 _ H1).  *)
+(*       rewrite dom_filter_comm. apply elem_of_filter. split; set_solver. } *)
+(*     iFrame "PMP". do 3 iModIntro. iFrame. *)
+(*     iSplitL "FUELS". *)
+(*     { solve_fuels_S FS. }  *)
+(*     iIntros "ST FUELS".  *)
 
-    simpl. iApply wp_value'.
-    iMod ("CLOS" with "[ST YST_AUTH inv']") as "_".
-    { rewrite /client_inv_impl. iNext. iExists (_, _). iFrame. }
-    iModIntro. iApply "POST".
-    iDestruct (has_fuels_equiv with "FUELS") as "[MAP FUEL]".
-    iApply partial_mapping_is_Proper; [| by iFrame].
-    f_equiv. rewrite map_fmap_singleton dom_singleton_L.
-    rewrite difference_diag_L. 
-    rewrite dom_filter_comm.
-    by rewrite dom_singleton_L filter_singleton_not.  
-  Qed. 
+(*     simpl. iApply wp_value'. *)
+(*     iMod ("CLOS" with "[ST YST_AUTH inv']") as "_". *)
+(*     { rewrite /client_inv_impl. iNext. iExists (_, _). iFrame. } *)
+(*     iModIntro. iApply "POST". *)
+(*     iDestruct (has_fuels_equiv with "FUELS") as "[MAP FUEL]". *)
+(*     iApply partial_mapping_is_Proper; [| by iFrame]. *)
+(*     f_equiv. rewrite map_fmap_singleton dom_singleton_L. *)
+(*     rewrite difference_diag_L.  *)
+(*     rewrite dom_filter_comm. *)
+(*     by rewrite dom_singleton_L filter_singleton_not.   *)
+(*   Qed.  *)
   
  
-End ClientSpec.
+(* End ClientSpec. *)
